add BBSrem sat and etc

src/BBSdiv.v
@@ -46,7 +46,7 @@ Definition bit_blast_sdiv g ls1 ls2 : generator * cnf * word * word :=
   let '(g_abs2, cs_abs2, lrs_abs2) := bit_blast_abs g_abs1 ls2 in
   let '(g_udiv, cs_udiv, qs_udiv, rs_udiv) := bit_blast_udiv g_abs2 lrs_abs1 lrs_abs2 in
   if (ls1_sign == lit_ff) && (ls2_sign == lit_ff) then
-    (g_udiv, catrev cs_udiv (catrev cs_abs1 cs_abs2), qs_udiv, rs_udiv)
+    (g_udiv, catrev (catrev cs_abs1 cs_abs2) cs_udiv, qs_udiv, rs_udiv)
   else if  (ls1_sign == lit_tt) && (ls2_sign == lit_tt) then
          let '(g_negr, cs_negr, lrs_negr) := bit_blast_neg g_udiv rs_udiv in
          (g_negr, catrev (catrev (catrev cs_abs1 cs_abs2) cs_udiv) cs_negr, qs_udiv, lrs_negr)
@@ -77,7 +77,7 @@ Definition bit_blast_sdiv_sdiv g ls1 ls2 : generator * cnf * word :=
   let '(g_abs2, cs_abs2, lrs_abs2) := bit_blast_abs g_abs1 ls2 in
   let '(g_udiv, cs_udiv, qs_udiv, rs_udiv) := bit_blast_udiv g_abs2 lrs_abs1 lrs_abs2 in
   if (((ls1_sign == lit_ff) && (ls2_sign == lit_ff)) || ((ls1_sign == lit_tt) && (ls2_sign == lit_tt))) then
-    (g_udiv, catrev cs_udiv (catrev cs_abs1 cs_abs2), qs_udiv)
+    (g_udiv, catrev (catrev cs_abs1 cs_abs2) cs_udiv, qs_udiv)
   else if (((ls1_sign == lit_ff) && (ls2_sign == lit_tt)) || ((ls1_sign == lit_tt) && (ls2_sign == lit_ff))) then
          let '(g_negq, cs_negq, lrs_negq) := bit_blast_neg g_udiv qs_udiv in
          (g_negq, catrev (catrev (catrev cs_abs1 cs_abs2) cs_udiv) cs_negq, lrs_negq)
@@ -97,7 +97,7 @@ Definition bit_blast_srem g ls1 ls2 : generator * cnf * word :=
   let '(g_abs1, cs_abs1, lrs_abs1) := bit_blast_abs g ls1 in
   let '(g_abs2, cs_abs2, lrs_abs2) := bit_blast_abs g_abs1 ls2 in
   let '(g_udiv, cs_udiv, qs_udiv, rs_udiv) := bit_blast_udiv g_abs2 lrs_abs1 lrs_abs2 in
-  if (ls1_sign == lit_ff) then (g_udiv, catrev cs_udiv (catrev cs_abs1 cs_abs2), rs_udiv)
+  if (ls1_sign == lit_ff) then (g_udiv, catrev (catrev cs_abs1 cs_abs2) cs_udiv, rs_udiv)
   else if (ls1_sign == lit_tt) then
          let '(g_negr, cs_negr, lrs_negr) := bit_blast_neg g_udiv rs_udiv in
          (g_negr, catrev (catrev (catrev cs_abs1 cs_abs2) cs_udiv) cs_negr, lrs_negr)
@@ -111,7 +111,7 @@ Definition mk_env_abs E g ls : env * generator * cnf * word :=
   let (ls_tl, ls_sign) := eta_expand (splitmsl ls) in
   if (ls_sign == lit_tt) then  mk_env_neg E g ls
   else if (ls_sign == lit_ff) then (E, g, [::], ls)
-       else let ws := copy (size ls_tl) ls_sign in
+       else let ws := copy (size ls) ls_sign in
             let '(E_xor, g_xor, cs_xor, rs_xor) := mk_env_xor E g ls ws in
             let '(E_zext, g_zext, cs_zext, rs_zext) := mk_env_zeroextend (size ls_tl) E_xor g_xor (ls_sign::nil) in 
             let '(E_add, g_add, cs_add, rs_add) := mk_env_add E_zext g_zext rs_xor rs_zext in
@@ -120,22 +120,22 @@ Definition mk_env_abs E g ls : env * generator * cnf * word :=
 Definition mk_env_sdiv E g ls1 ls2 : env * generator * cnf * word * word :=
   let (ls1_tl, ls1_sign) := eta_expand (splitmsl ls1) in
   let (ls2_tl, ls2_sign) := eta_expand (splitmsl ls2) in
-  let ws1 := copy (size ls1_tl) ls1_sign in
+  let ws1 := copy (size ls1) ls1_sign in
   let '(E_abs1, g_abs1, cs_abs1, lrs_abs1) := mk_env_abs E g ls1 in
   let '(E_abs2, g_abs2, cs_abs2, lrs_abs2) := mk_env_abs E_abs1 g_abs1 ls2 in
   let '(E_udiv, g_udiv, cs_udiv, qs_udiv, rs_udiv) := mk_env_udiv E_abs2 g_abs2 lrs_abs1 lrs_abs2 in
   if (ls1_sign == lit_ff) && (ls1_sign == lit_ff) then
-    (E_udiv, g_udiv, catrev cs_udiv (catrev cs_abs1 cs_abs2), qs_udiv, rs_udiv)
+    (E_udiv, g_udiv, catrev (catrev cs_abs1 cs_abs2) cs_udiv, qs_udiv, rs_udiv)
   else if (ls1_sign == lit_tt) && (ls1_sign == lit_tt) then
          let '(E_negr, g_negr, cs_negr, lrs_negr) := mk_env_neg E_udiv g_udiv rs_udiv in
-         (E_negr, g_negr, catrev cs_negr (catrev cs_udiv (catrev cs_abs1 cs_abs2)), qs_udiv, lrs_negr)
+         (E_negr, g_negr, catrev (catrev  (catrev cs_abs1 cs_abs2) cs_udiv) cs_negr, qs_udiv, lrs_negr)
        else if (ls1_sign == lit_ff) && (ls1_sign == lit_tt) then
               let '(E_negq, g_negq, cs_negq, lrs_negq) := mk_env_neg E_udiv g_udiv qs_udiv in
               (E_negq, g_negq, catrev (catrev (catrev cs_abs1 cs_abs2) cs_udiv) cs_negq, lrs_negq, rs_udiv)
                 else if (ls1_sign == lit_tt) && (ls2_sign == lit_ff) then
                        let '(E_negq, g_negq, cs_negq, lrs_negq) := mk_env_neg E_udiv g_udiv qs_udiv in
                        let '(E_negr, g_negr, cs_negr, lrs_negr) := mk_env_neg E_negq g_negq rs_udiv in
-                       (E_negr, g_negr, catrev cs_negr (catrev cs_negq (catrev cs_udiv (catrev cs_abs1 cs_abs2))), lrs_negq, lrs_negr)
+                       (E_negr, g_negr, catrev (catrev (catrev (catrev cs_abs1 cs_abs2) cs_udiv) cs_negq) cs_negr, lrs_negq, lrs_negr)
             else 
               let '(E_eq, g_eq, cs_eq, r_eq) := mk_env_eq E_udiv g_udiv (ls1_sign::nil) (ls2_sign::nil) in
               let '(E_lneg, g_lneg, cs_lneg, r_lneg) := mk_env_lneg E_eq g_eq r_eq in
@@ -151,7 +151,7 @@ Definition mk_env_sdiv E g ls1 ls2 : env * generator * cnf * word * word :=
 Definition mk_env_sdiv_sdiv E g ls1 ls2 : env * generator * cnf * word :=
   let (ls1_tl, ls1_sign) := eta_expand (splitmsl ls1) in
   let (ls2_tl, ls2_sign) := eta_expand (splitmsl ls2) in
-  let ws1 := copy (size ls1_tl) ls1_sign in
+  let ws1 := copy (size ls1) ls1_sign in
   let '(E_abs1, g_abs1, cs_abs1, lrs_abs1) := mk_env_abs E g ls1 in
   let '(E_abs2, g_abs2, cs_abs2, lrs_abs2) := mk_env_abs E_abs1 g_abs1 ls2 in
   let '(E_udiv, g_udiv, cs_udiv, qs_udiv, rs_udiv) := mk_env_udiv E_abs2 g_abs2 lrs_abs1 lrs_abs2 in
@@ -172,15 +172,15 @@ Definition mk_env_sdiv_sdiv E g ls1 ls2 : env * generator * cnf * word :=
 Definition mk_env_srem E g ls1 ls2 : env * generator * cnf * word :=
   let (ls1_tl, ls1_sign) := eta_expand (splitmsl ls1) in
   (*let (ls2_tl, ls2_sign) := eta_expand (splitmsl ls2) in*)
-  let ws1 := copy (size ls1_tl) ls1_sign in
+  let ws1 := copy (size ls1) ls1_sign in
   let '(E_abs1, g_abs1, cs_abs1, lrs_abs1) := mk_env_abs E g ls1 in
   let '(E_abs2, g_abs2, cs_abs2, lrs_abs2) := mk_env_abs E_abs1 g_abs1 ls2 in
   let '(E_udiv, g_udiv, cs_udiv, qs_udiv, rs_udiv) := mk_env_udiv E_abs2 g_abs2 lrs_abs1 lrs_abs2 in
   if (ls1_sign == lit_ff) then
-    (E_udiv, g_udiv, catrev cs_udiv (catrev cs_abs1 cs_abs2), rs_udiv)
+    (E_udiv, g_udiv, catrev (catrev cs_abs1 cs_abs2) cs_udiv, rs_udiv)
   else if (ls1_sign == lit_tt) then
          let '(E_negr, g_negr, cs_negr, lrs_negr) := mk_env_neg E_udiv g_udiv rs_udiv in
-         (E_negr, g_negr, catrev cs_negr (catrev cs_udiv (catrev cs_abs1 cs_abs2)), lrs_negr)
+         (E_negr, g_negr, catrev (catrev (catrev cs_abs1 cs_abs2) cs_udiv) cs_negr, lrs_negr)
        else 
          let '(E_xor1, g_xor1, cs_xor1, rs_xor1) := mk_env_xor E_udiv g_udiv rs_udiv ws1 in
          let '(E_zext1, g_zext1, cs_zext1, rs_zext1) := mk_env_zeroextend (size ls1_tl) E_xor1 g_xor1 (ls1_sign::nil) in
@@ -285,7 +285,7 @@ Proof.
 Qed.
  *)
 
-Lemma bits_v1_cons_zoros bs :
+Lemma bits_v1_cons_zeros bs :
   0 < size bs ->
   (true :: copy (size bs - 1) b0) = (size (invB bs)) -bits of (1)%bits.
 Proof.
@@ -393,12 +393,12 @@ Proof.
     move : (bit_blast_neg_correct Hbbneg1 Hencr Hcsneg1).
     rewrite -/(msb bs2) xorBC xorB_copy_case size_splitmsb.  
     generalize Hsz2; rewrite Hszlb2; move => Hszgt02. case Hms2 : (msb bs2).
-    rewrite (bits_v1_cons_zoros Hszgt02) addB1 -/(negB bs2)//.
+    rewrite (bits_v1_cons_zeros Hszgt02) addB1 -/(negB bs2)//.
     rewrite /= zeros_cons subn1 (ltn_predK Hszgt02) addB0 unzip1_zip//; last by rewrite size_zeros.
   - dcase (bit_blast_neg g ls2) => [[[g_neg2] cs_neg2] lrs_neg2] Hbbneg2.
     dcase (bit_blast_udiv g_neg2 ls1 lrs_neg2)=> [[[[g_udiv] cs_udiv] lqs_udiv] lrs_udiv] Hbbudiv.
     case => _ <- <-. move => Hsz12 Hsz2 Henc1 Henc2.
-    rewrite !add_prelude_catrev. move/andP => [Hcsu Hcsneg2]. 
+    rewrite !add_prelude_catrev. move/andP => [Hcsneg2 Hcsu]. 
     move : (bit_blast_neg_correct Hbbneg2 Henc2 Hcsneg2) => Hencneg2.
     generalize Hsz12. rewrite (bit_blast_neg_size_ss Hbbneg2). move => Hszneg2.
     move : (bit_blast_udiv_correct Hbbudiv Hszneg2 Henc1 Hencneg2 Hcsu)=> [_ Hencr].
@@ -412,7 +412,7 @@ Proof.
     rewrite /sremB /absB -Hmsb2t Hmsb1f//.
   - dcase (bit_blast_udiv g ls1 ls2 ) =>[[[[g_udiv] cs_udiv] qs_udiv] rs_udiv] Hbbudiv.
     case => _ <- <-. move => Hsz12 Hsz2 Henc1 Henc2.
-    rewrite add_prelude_catrev. move/andP => [Hcsu _].
+    (*rewrite add_prelude_catrev.*) move => Hcsu.
     move : (add_prelude_tt Hcsu) => Htt.
     move : (enc_bit_msb Htt Henc1). rewrite/msl (eqP Hls1mb0). move => Hencmsb1.
     move : (enc_bit_msb Htt Henc2). rewrite/msl (eqP Hls2mb0). move => Hencmsb2.
@@ -427,7 +427,7 @@ Proof.
     dcase (bit_blast_add g_xor1 lrs_xor1 ((splitmsl ls2).2 :: copy (size (splitmsl ls2).1) lit_ff)) => [[[g_add1] cs_add1] lrs_add1] Hbbadd1.
     dcase (bit_blast_udiv g_add1 ls1 lrs_add1) =>[[[[g_udiv] cs_udiv] qs_udiv] rs_udiv] Hbbudiv.
     case => _ <- <-. move => Hsz12 Hsz2 Henc1 Henc2.
-    rewrite 3!add_prelude_catrev/=. move/andP => [Hcsudiv Hcsu]; move/andP : Hcsu => [Hcsu Hcsadd1].
+    rewrite 3!add_prelude_catrev/=. move/andP => [Hcsu Hcsudiv]; move/andP : Hcsu => [Hcsu Hcsadd1].
     move/andP : Hcsu => [Hcsxor1 _].
     move : (add_prelude_tt Hcsudiv) => Htt.
     move : (enc_bit_msb Htt Henc1); rewrite/msl (eqP Hls1mb0); move => Hencmsb1.
@@ -451,7 +451,7 @@ Proof.
     move : (bit_blast_udiv_correct Hbbudiv Hsz1add1 Henc1 Hencadd1 Hcsudiv) => [_ Hencr].
     move : Hencr; rewrite -/(msb bs2) xorBC xorB_copy_case size_splitmsb.
     generalize Hsz2; rewrite Hszlb2; move => Hszgt02. case Hms2 : (msb bs2).
-    rewrite (bits_v1_cons_zoros Hszgt02) addB1 -/(negB bs2)//.
+    rewrite (bits_v1_cons_zeros Hszgt02) addB1 -/(negB bs2)//.
     rewrite /= zeros_cons subn1 (ltn_predK Hszgt02) addB0 unzip1_zip//; last by rewrite size_zeros.
   - rewrite (lock splitmsl) /= -!lock.
     dcase (bit_blast_neg g_add ls2) => [[[g_neg1] cs_neg1] lrs_neg1] Hbbneg1.
@@ -503,7 +503,7 @@ Proof.
     have Hszdiv : size bs1 = size ((udivB (bs1 ^# copy (size bs1) true +# zext (size ls1 - 1) [:: true]) (-# bs2)).2)%bits.
     by rewrite size_uremB size_addB size_xorB size_copy size_zext addnC/=(subnK Hsz1) Hszlb1 maxnn minnn//.
     generalize Hsz1; rewrite Hszlb1; move => Hszgt01. case Hmsb1 : (msb bs1).
-    + rewrite xorBC {1}Hszdiv (xorBC bs1 (copy (size bs1) true)) Hszlb1 2!xorB_copy_case -/b0 (bits_v1_cons_zoros Hszgt01) (bits_v1_zext_b1 Hszgt01).
+    + rewrite xorBC {1}Hszdiv (xorBC bs1 (copy (size bs1) true)) Hszlb1 2!xorB_copy_case -/b0 (bits_v1_cons_zeros Hszgt01) (bits_v1_zext_b1 Hszgt01).
       move => {Hszdiv}.
       have {2}-> : size (~~# bs1)%bits = size (~~# (udivB (~~# bs1 +# (size (~~# bs1)) -bits of (1)) (-# bs2)).2)%bits.
         by rewrite !size_invB size_uremB size_addB size_invB size_from_nat minnn.
@@ -555,7 +555,7 @@ Proof.
     move : (bit_blast_add_correct Hbbadd2 Hencxor2 Henccpcmsb1 Hadd2rs Hcsadd2 Hszu).
     rewrite -/(msb bs1) size_splitmsl size_splitmsb Hszlb1 (xorBC bs1 (copy (size bs1) (msb bs1))) xorB_copy_case.
     generalize Hsz1; rewrite Hszlb1; move => Hszgt0. case Hmsb1 : (msb bs1).
-    + rewrite (bits_v1_zext_b1 Hszgt0) addB1 -/(negB _) -{1}(size_negB bs1) -{1}(size_uremB (-#bs1)%bits (bs2)) xorBC xorB_copy_case (bits_v1_cons_zoros Hszgt0).
+    + rewrite (bits_v1_zext_b1 Hszgt0) addB1 -/(negB _) -{1}(size_negB bs1) -{1}(size_uremB (-#bs1)%bits (bs2)) xorBC xorB_copy_case (bits_v1_cons_zeros Hszgt0).
       rewrite size_invB -{1}(size_negB bs1) -{1}(size_uremB (-#bs1)%bits (bs2)) -(size_invB _) addB1 -/(negB _)//.
     + have {1}->: [:: false] = zeros 1 by done.
       rewrite zext_zero -/(zeros (size bs1 -1)) zeros_cons -(addn1 (size bs1 -1)) (subnK Hszgt0).
@@ -617,12 +617,12 @@ Proof.
     generalize Hsz1; rewrite Hszlb1; move => Hszgt0; generalize Hszgt0; rewrite {1}Hszb12; move => Hszgt02.
     rewrite -/(msb bs1) -/(msb bs2) xorBC (xorBC bs1 (copy (size bs1) (msb bs1))) (xorBC bs2 (copy (size bs2) (msb bs2))) size_splitmsl !size_splitmsb {1}Hszlb1.
     case Hmsb1 : (msb bs1); case Hmsb2 : (msb bs2); rewrite 2!xorB_copy_case//.
-    + rewrite (bits_v1_cons_zoros Hszgt02) (bits_v1_zext_b1 Hszgt0) 2!addB1 -2!/(negB _) (bits_v1_cons_zoros Hszgt0).
+    + rewrite (bits_v1_cons_zeros Hszgt02) (bits_v1_zext_b1 Hszgt0) 2!addB1 -2!/(negB _) (bits_v1_cons_zeros Hszgt0).
       rewrite size_invB -{1 2}(size_negB _) -(size_uremB (-#bs1)%bits (-#bs2)%bits) xorB_copy_case -(size_invB _) addB1 -/(negB _)//.
     + rewrite (bits_v1_zext_b1 Hszgt0) zeros_cons subn1 (ltn_predK Hszgt02) addB0 unzip1_zip; last by rewrite size_zeros.
-      rewrite addB1 -/(negB _) -{1}(size_negB bs1) -{1}(size_uremB (-#bs1)%bits bs2) xorB_copy_case (bits_v1_cons_zoros Hszgt0).
+      rewrite addB1 -/(negB _) -{1}(size_negB bs1) -{1}(size_uremB (-#bs1)%bits bs2) xorB_copy_case (bits_v1_cons_zeros Hszgt0).
       rewrite size_invB -{1}(size_negB bs1) -{1}(size_uremB (-#bs1)%bits bs2) -(size_invB _) addB1 -/(negB _)//.
-    + have -> : [::false] = zeros 1 by done. rewrite zext_zero (bits_v1_cons_zoros Hszgt02) addB1 (subnK Hszgt0) -/(negB _).
+    + have -> : [::false] = zeros 1 by done. rewrite zext_zero (bits_v1_cons_zeros Hszgt02) addB1 (subnK Hszgt0) -/(negB _).
       rewrite zeros_cons !addB0 !unzip1_zip;
         [rewrite -(size_uremB bs1 (-#bs2)%bits) xorB_copy_case//|rewrite size_zeros//
          |rewrite size_xorB /zeros !size_copy size_uremB subn1 (ltn_predK Hszgt0) maxnn//|rewrite size_zeros//].
@@ -631,7 +631,878 @@ Proof.
       rewrite -(size_uremB bs1 bs2) xorB_copy_case//.
 Qed.
 
-(* Lemma bit_blast_sdiv_correct g ls1 ls2 g' cs qlrs rlrs E bs1 bs2 : *)
+Lemma mk_env_srem_is_bit_blast_srem : forall ls1 E g ls2 g' cs rlrs E',
+  mk_env_srem E g ls1 ls2 = (E', g', cs, rlrs) ->
+  bit_blast_srem g ls1 ls2  = (g', cs, rlrs).
+Proof.
+  rewrite /bit_blast_srem /mk_env_srem /bit_blast_abs /mk_env_abs.
+  move => ls1 E g ls2 g' cs rlrs E'.
+  dcase (mk_env_neg E g ls1) => [[[[E_neg1] g_neg1] cs_neg1] rs_neg1] Hmkneg1.
+  dcase (mk_env_xor E g ls1 (copy (size ls1) (splitmsl ls1).2)) => [[[[E_xor1] g_xor1] cs_xor1] rs_xor1] Hmkxor1.
+  dcase (mk_env_zeroextend (size (splitmsl ls1).1) E_xor1 g_xor1 [:: (splitmsl ls1).2]) => [[[[E_zext1] g_zext1] cs_zext1] rs_zext1] Hmkzext1.
+  dcase (mk_env_add E_zext1 g_zext1 rs_xor1 rs_zext1) => [[[[E_add] g_add] cs_add] rs_add] Hmkadd1.
+  rewrite (mk_env_neg_is_bit_blast_neg Hmkneg1) (mk_env_xor_is_bit_blast_xor Hmkxor1) (mk_env_zeroextend_is_bit_blast_zeroextend Hmkzext1) (mk_env_add_is_bit_blast_add Hmkadd1).
+  case Htt1: ((splitmsl ls1).2 == lit_tt); case Hff1 : ((splitmsl ls1).2 == lit_ff);
+    case Htt2 : ((splitmsl ls2).2 == lit_tt); case Hff2 : ((splitmsl ls2).2 == lit_ff);
+      try rewrite (eqP Htt1)// in Hff1; try rewrite (eqP Htt2)// in Hff2.
+  - dcase (mk_env_neg E_neg1 g_neg1 ls2) => [[[[E_abs2] g_abs2] cs_abs2] lrs_abs2] Hmkneg2.
+    dcase (mk_env_udiv E_abs2 g_abs2 rs_neg1 lrs_abs2) => [[[[[E_udiv] g_udiv] cs_udiv] lqs_udiv]lrs_udiv] Hmkudiv.
+    dcase (mk_env_neg E_udiv g_udiv lrs_udiv) => [[[[E_negr] g_negr] cs_negr] lrs_negr] Hmknegr.
+    rewrite (mk_env_neg_is_bit_blast_neg Hmkneg2) (mk_env_udiv_is_bit_blast_udiv Hmkudiv) (mk_env_neg_is_bit_blast_neg Hmknegr); case => _ <- <- <- //.
+  - dcase (mk_env_udiv E_neg1 g_neg1 rs_neg1 ls2) => [[[[[E_udiv] g_udiv] cs_udiv] lqs_udiv]lrs_udiv] Hmkudiv.
+    dcase (mk_env_neg E_udiv g_udiv lrs_udiv) => [[[[E_negr] g_negr] cs_negr] lrs_negr] Hmknegr.
+    rewrite (mk_env_udiv_is_bit_blast_udiv Hmkudiv) (mk_env_neg_is_bit_blast_neg Hmknegr); case => _ <- <- <- //.
+  - dcase (mk_env_xor E_neg1 g_neg1 ls2 (copy (size ls2) (splitmsl ls2).2)) => [[[[E_xor2] g_xor2] cs_xor2] rs_xor2] Hmkxor2.
+    dcase (mk_env_zeroextend (size (splitmsl ls2).1) E_xor2 g_xor2 [:: (splitmsl ls2).2]) => [[[[E_zext2] g_zext2] cs_zext2] rs_zext2] Hmkzext2.
+    dcase (mk_env_add E_zext2 g_zext2 rs_xor2 rs_zext2) => [[[[E_add2] g_add2] cs_add2] rs_add2] Hmkadd2.
+    dcase (mk_env_udiv E_add2 g_add2 rs_neg1 rs_add2) => [[[[[E_udiv] g_udiv] cs_udiv] lqs_udiv] lrs_udiv] Hmkudiv.
+    dcase (mk_env_neg E_udiv g_udiv lrs_udiv) => [[[[E_negr] g_negr] cs_negr] lrs_negr] Hmknegr.
+    rewrite (mk_env_xor_is_bit_blast_xor Hmkxor2) (mk_env_zeroextend_is_bit_blast_zeroextend Hmkzext2) (mk_env_add_is_bit_blast_add Hmkadd2) (mk_env_udiv_is_bit_blast_udiv Hmkudiv) (mk_env_neg_is_bit_blast_neg Hmknegr); case => _ <- <- <- //.
+  - dcase (mk_env_neg E g ls2) => [[[[E_abs2] g_abs2] cs_abs2] lrs_abs2] Hmkneg2.
+    dcase (mk_env_udiv E_abs2 g_abs2 ls1 lrs_abs2) => [[[[[E_udiv] g_udiv] cs_udiv] lqs_udiv]lrs_udiv] Hmkudiv.
+    rewrite (mk_env_neg_is_bit_blast_neg Hmkneg2) (mk_env_udiv_is_bit_blast_udiv Hmkudiv); case => _ <- <- <- //.
+  - dcase (mk_env_udiv E g ls1 ls2) => [[[[[E_udiv] g_udiv] cs_udiv] lqs_udiv]lrs_udiv] Hmkudiv.
+    rewrite (mk_env_udiv_is_bit_blast_udiv Hmkudiv); case => _ <- <- <- //.
+  - dcase (mk_env_xor E g ls2 (copy (size ls2) (splitmsl ls2).2)) => [[[[E_xor2] g_xor2] cs_xor2] rs_xor2] Hmkxor2.
+    dcase (mk_env_zeroextend (size (splitmsl ls2).1) E_xor2 g_xor2 [:: (splitmsl ls2).2]) => [[[[E_zext2] g_zext2] cs_zext2] rs_zext2] Hmkzext2.
+    dcase (mk_env_add E_zext2 g_zext2 rs_xor2 rs_zext2) => [[[[E_add2] g_add2] cs_add2] rs_add2] Hmkadd2.
+    dcase (mk_env_udiv E_add2 g_add2 ls1 rs_add2) => [[[[[E_udiv] g_udiv] cs_udiv] lqs_udiv] lrs_udiv] Hmkudiv.
+    rewrite (mk_env_xor_is_bit_blast_xor Hmkxor2) (mk_env_zeroextend_is_bit_blast_zeroextend Hmkzext2) (mk_env_add_is_bit_blast_add Hmkadd2) (mk_env_udiv_is_bit_blast_udiv Hmkudiv); case => _ <- <- <- //.
+  - dcase (mk_env_neg E_add g_add ls2) => [[[[E_abs2] g_abs2] cs_abs2] lrs_abs2] Hmkneg2.
+    dcase (mk_env_udiv E_abs2 g_abs2 rs_add lrs_abs2) => [[[[[E_udiv] g_udiv] cs_udiv] lqs_udiv]lrs_udiv] Hmkudiv.
+    dcase (mk_env_xor E_udiv g_udiv lrs_udiv (copy (size ls1) (splitmsl ls1).2)) => [[[[E_xorr] g_xorr] cs_xorr] rs_xorr] Hmkxorr.
+    dcase (mk_env_zeroextend (size (splitmsl ls1).1) E_xorr g_xorr [:: (splitmsl ls1).2]) => [[[[E_zextr] g_zextr] cs_zextr] rs_zextr] Hmkzextr.
+    dcase (mk_env_add E_zextr g_zextr rs_xorr rs_zextr) => [[[[E_addr] g_addr] cs_addr] rs_addr] Hmkaddr.
+    rewrite (mk_env_neg_is_bit_blast_neg Hmkneg2) (mk_env_udiv_is_bit_blast_udiv Hmkudiv) (mk_env_xor_is_bit_blast_xor Hmkxorr) (mk_env_zeroextend_is_bit_blast_zeroextend Hmkzextr) (mk_env_add_is_bit_blast_add Hmkaddr); case => _ <- <- <- //.
+  - dcase (mk_env_udiv E_add g_add rs_add ls2) => [[[[[E_udiv] g_udiv] cs_udiv] lqs_udiv]lrs_udiv] Hmkudiv.
+    dcase (mk_env_xor E_udiv g_udiv lrs_udiv (copy (size ls1) (splitmsl ls1).2)) => [[[[E_xorr] g_xorr] cs_xorr] rs_xorr] Hmkxorr.
+    dcase (mk_env_zeroextend (size (splitmsl ls1).1) E_xorr g_xorr [:: (splitmsl ls1).2]) => [[[[E_zextr] g_zextr] cs_zextr] rs_zextr] Hmkzextr.
+    dcase (mk_env_add E_zextr g_zextr rs_xorr rs_zextr) => [[[[E_addr] g_addr] cs_addr] rs_addr] Hmkaddr.
+    rewrite (mk_env_udiv_is_bit_blast_udiv Hmkudiv) (mk_env_xor_is_bit_blast_xor Hmkxorr) (mk_env_zeroextend_is_bit_blast_zeroextend Hmkzextr) (mk_env_add_is_bit_blast_add Hmkaddr); case => _ <- <- <- //.
+  - dcase (mk_env_xor E_add g_add ls2 (copy (size ls2) (splitmsl ls2).2)) => [[[[E_xor2] g_xor2] cs_xor2] rs_xor2] Hmkxor2.
+    dcase (mk_env_zeroextend (size (splitmsl ls2).1) E_xor2 g_xor2 [:: (splitmsl ls2).2]) => [[[[E_zext2] g_zext2] cs_zext2] rs_zext2] Hmkzext2.
+    dcase (mk_env_add E_zext2 g_zext2 rs_xor2 rs_zext2) => [[[[E_abs2] g_abs2] cs_abs2] lrs_abs2] Hmkadd2.
+    dcase (mk_env_udiv E_abs2 g_abs2 rs_add lrs_abs2) => [[[[[E_udiv] g_udiv] cs_udiv] lqs_udiv]lrs_udiv] Hmkudiv.
+    dcase (mk_env_xor E_udiv g_udiv lrs_udiv (copy (size ls1) (splitmsl ls1).2)) => [[[[E_xorr] g_xorr] cs_xorr] rs_xorr] Hmkxorr.
+    dcase (mk_env_zeroextend (size (splitmsl ls1).1) E_xorr g_xorr [:: (splitmsl ls1).2]) => [[[[E_zextr] g_zextr] cs_zextr] rs_zextr] Hmkzextr.
+    dcase (mk_env_add E_zextr g_zextr rs_xorr rs_zextr) => [[[[E_addr] g_addr] cs_addr] rs_addr] Hmkaddr.
+    rewrite (mk_env_xor_is_bit_blast_xor Hmkxor2) (mk_env_zeroextend_is_bit_blast_zeroextend Hmkzext2) (mk_env_add_is_bit_blast_add Hmkadd2) (mk_env_udiv_is_bit_blast_udiv Hmkudiv) (mk_env_xor_is_bit_blast_xor Hmkxorr) (mk_env_zeroextend_is_bit_blast_zeroextend Hmkzextr) (mk_env_add_is_bit_blast_add Hmkaddr); case => _ <- <- <- //.
+Qed.
+
+Lemma mk_env_srem_newer_gen :
+  forall ls1 E g ls2 E' g' cs lrs,
+    mk_env_srem E g ls1 ls2 = (E', g', cs, lrs) ->
+    (g <=? g')%positive.
+Proof.
+  rewrite /mk_env_srem /mk_env_abs. move => ls1 E g ls2 E' g' cs lrs.
+  dcase (mk_env_neg E g ls1) => [[[[E_neg1] g_neg1] cs_neg1] rs_neg1] Hmkneg1.
+  dcase (mk_env_xor E g ls1 (copy (size ls1) (splitmsl ls1).2)) => [[[[E_xor1] g_xor1] cs_xor1] rs_xor1] Hmkxor1.
+  dcase (mk_env_zeroextend (size (splitmsl ls1).1) E_xor1 g_xor1 [:: (splitmsl ls1).2]) => [[[[E_zext1] g_zext1] cs_zext1] rs_zext1] Hmkzext1.
+  dcase (mk_env_add E_zext1 g_zext1 rs_xor1 rs_zext1) => [[[[E_add] g_add] cs_add] rs_add] Hmkadd1.
+  move : (mk_env_neg_newer_gen Hmkneg1) => Hnewneg1.
+  move : (mk_env_xor_newer_gen Hmkxor1) => Hnewxor1.
+  move : (mk_env_zeroextend_newer_gen Hmkzext1) => Hnewzext1.
+  move : (mk_env_add_newer_gen Hmkadd1) => Hnewadd1.
+  move : (pos_leb_trans Hnewxor1 (pos_leb_trans Hnewzext1 Hnewadd1)) => Hnegls1.
+  case Htt1: ((splitmsl ls1).2 == lit_tt); case Hff1 : ((splitmsl ls1).2 == lit_ff);
+    case Htt2 : ((splitmsl ls2).2 == lit_tt); case Hff2 : ((splitmsl ls2).2 == lit_ff);
+      try rewrite (eqP Htt1)// in Hff1; try rewrite (eqP Htt2)// in Hff2.
+  - dcase (mk_env_neg E_neg1 g_neg1 ls2) => [[[[E_abs2] g_abs2] cs_abs2] lrs_abs2] Hmkneg2.
+    dcase (mk_env_udiv E_abs2 g_abs2 rs_neg1 lrs_abs2) => [[[[[E_udiv] g_udiv] cs_udiv] lqs_udiv]lrs_udiv] Hmkudiv.
+    dcase (mk_env_neg E_udiv g_udiv lrs_udiv) => [[[[E_negr] g_negr] cs_negr] lrs_negr] Hmknegr.
+    move : (mk_env_neg_newer_gen Hmkneg2) => Hnewneg2.
+    move : (mk_env_udiv_newer_gen Hmkudiv) => Hnewudiv.
+    move : (mk_env_neg_newer_gen Hmknegr) => Hnewnegr.
+    case => _ <- _ _ //; exact : (pos_leb_trans Hnewneg1 (pos_leb_trans Hnewneg2 (pos_leb_trans Hnewudiv Hnewnegr))).
+  - dcase (mk_env_udiv E_neg1 g_neg1 rs_neg1 ls2) => [[[[[E_udiv] g_udiv] cs_udiv] lqs_udiv]lrs_udiv] Hmkudiv.
+    dcase (mk_env_neg E_udiv g_udiv lrs_udiv) => [[[[E_negr] g_negr] cs_negr] lrs_negr] Hmknegr.
+    move : (mk_env_udiv_newer_gen Hmkudiv) => Hnewudiv.
+    move : (mk_env_neg_newer_gen Hmknegr) => Hnewnegr.
+    case => _ <- _ _ //; exact : (pos_leb_trans Hnewneg1 (pos_leb_trans Hnewudiv Hnewnegr)).
+  - dcase (mk_env_xor E_neg1 g_neg1 ls2 (copy (size ls2) (splitmsl ls2).2)) => [[[[E_xor2] g_xor2] cs_xor2] rs_xor2] Hmkxor2.
+    dcase (mk_env_zeroextend (size (splitmsl ls2).1) E_xor2 g_xor2 [:: (splitmsl ls2).2]) => [[[[E_zext2] g_zext2] cs_zext2] rs_zext2] Hmkzext2.
+    dcase (mk_env_add E_zext2 g_zext2 rs_xor2 rs_zext2) => [[[[E_add2] g_add2] cs_add2] rs_add2] Hmkadd2.
+    dcase (mk_env_udiv E_add2 g_add2 rs_neg1 rs_add2) => [[[[[E_udiv] g_udiv] cs_udiv] lqs_udiv] lrs_udiv] Hmkudiv.
+    dcase (mk_env_neg E_udiv g_udiv lrs_udiv) => [[[[E_negr] g_negr] cs_negr] lrs_negr] Hmknegr.
+    move : (mk_env_xor_newer_gen Hmkxor2) => Hnewxor2.
+    move : (mk_env_zeroextend_newer_gen Hmkzext2) => Hnewzext2.
+    move : (mk_env_add_newer_gen Hmkadd2) => Hnewadd2.
+    move : (mk_env_udiv_newer_gen Hmkudiv) => Hnewudiv.
+    move : (mk_env_neg_newer_gen Hmknegr) => Hnewnegr.
+    case  => _ <- _ _ //; exact : (pos_leb_trans Hnewneg1 (pos_leb_trans Hnewxor2 (pos_leb_trans Hnewzext2 (pos_leb_trans Hnewadd2 (pos_leb_trans Hnewudiv Hnewnegr))))).
+  - dcase (mk_env_neg E g ls2) => [[[[E_abs2] g_abs2] cs_abs2] lrs_abs2] Hmkneg2.
+    dcase (mk_env_udiv E_abs2 g_abs2 ls1 lrs_abs2) => [[[[[E_udiv] g_udiv] cs_udiv] lqs_udiv]lrs_udiv] Hmkudiv.
+    move : (mk_env_neg_newer_gen Hmkneg2) => Hnewneg2.
+    move : (mk_env_udiv_newer_gen Hmkudiv) => Hnewudiv.
+    case  => _ <- _ _ //; exact : (pos_leb_trans Hnewneg2 Hnewudiv).
+  - dcase (mk_env_udiv E g ls1 ls2) => [[[[[E_udiv] g_udiv] cs_udiv] lqs_udiv]lrs_udiv] Hmkudiv.
+    case  => _ <- _ _ //; exact : (mk_env_udiv_newer_gen Hmkudiv).
+  - dcase (mk_env_xor E g ls2 (copy (size ls2) (splitmsl ls2).2)) => [[[[E_xor2] g_xor2] cs_xor2] rs_xor2] Hmkxor2.
+    dcase (mk_env_zeroextend (size (splitmsl ls2).1) E_xor2 g_xor2 [:: (splitmsl ls2).2]) => [[[[E_zext2] g_zext2] cs_zext2] rs_zext2] Hmkzext2.
+    dcase (mk_env_add E_zext2 g_zext2 rs_xor2 rs_zext2) => [[[[E_add2] g_add2] cs_add2] rs_add2] Hmkadd2.
+    dcase (mk_env_udiv E_add2 g_add2 ls1 rs_add2) => [[[[[E_udiv] g_udiv] cs_udiv] lqs_udiv] lrs_udiv] Hmkudiv.
+    move : (mk_env_xor_newer_gen Hmkxor2) => Hnewxor2.
+    move : (mk_env_zeroextend_newer_gen Hmkzext2) => Hnewzext2.
+    move : (mk_env_add_newer_gen Hmkadd2) => Hnewadd2.
+    move : (mk_env_udiv_newer_gen Hmkudiv) => Hnewudiv.
+    case  => _ <- _ _ //; exact : (pos_leb_trans Hnewxor2 (pos_leb_trans Hnewzext2 (pos_leb_trans Hnewadd2 Hnewudiv))).
+  - dcase (mk_env_neg E_add g_add ls2) => [[[[E_abs2] g_abs2] cs_abs2] lrs_abs2] Hmkneg2.
+    dcase (mk_env_udiv E_abs2 g_abs2 rs_add lrs_abs2) => [[[[[E_udiv] g_udiv] cs_udiv] lqs_udiv]lrs_udiv] Hmkudiv.
+    dcase (mk_env_xor E_udiv g_udiv lrs_udiv (copy (size ls1) (splitmsl ls1).2)) => [[[[E_xorr] g_xorr] cs_xorr] rs_xorr] Hmkxorr.
+    dcase (mk_env_zeroextend (size (splitmsl ls1).1) E_xorr g_xorr [:: (splitmsl ls1).2]) => [[[[E_zextr] g_zextr] cs_zextr] rs_zextr] Hmkzextr.
+    dcase (mk_env_add E_zextr g_zextr rs_xorr rs_zextr) => [[[[E_addr] g_addr] cs_addr] rs_addr] Hmkaddr.
+    move : (mk_env_neg_newer_gen Hmkneg2) => Hnewneg2.
+    move : (mk_env_udiv_newer_gen Hmkudiv) => Hnewudiv.
+    move : (mk_env_xor_newer_gen Hmkxorr) => Hnewxorr.
+    move : (mk_env_zeroextend_newer_gen Hmkzextr) => Hnewzextr.
+    move : (mk_env_add_newer_gen Hmkaddr) => Hnewaddr.
+    case  => _ <- _ _ //; exact : (pos_leb_trans Hnegls1 (pos_leb_trans Hnewneg2 (pos_leb_trans Hnewudiv (pos_leb_trans Hnewxorr (pos_leb_trans Hnewzextr Hnewaddr))))).
+  - dcase (mk_env_udiv E_add g_add rs_add ls2) => [[[[[E_udiv] g_udiv] cs_udiv] lqs_udiv]lrs_udiv] Hmkudiv.
+    dcase (mk_env_xor E_udiv g_udiv lrs_udiv (copy (size ls1) (splitmsl ls1).2)) => [[[[E_xorr] g_xorr] cs_xorr] rs_xorr] Hmkxorr.
+    dcase (mk_env_zeroextend (size (splitmsl ls1).1) E_xorr g_xorr [:: (splitmsl ls1).2]) => [[[[E_zextr] g_zextr] cs_zextr] rs_zextr] Hmkzextr.
+    dcase (mk_env_add E_zextr g_zextr rs_xorr rs_zextr) => [[[[E_addr] g_addr] cs_addr] rs_addr] Hmkaddr.
+    move : (mk_env_udiv_newer_gen Hmkudiv) => Hnewudiv.
+    move : (mk_env_xor_newer_gen Hmkxorr) => Hnewxorr.
+    move : (mk_env_zeroextend_newer_gen Hmkzextr) => Hnewzextr.
+    move : (mk_env_add_newer_gen Hmkaddr) => Hnewaddr.
+    case  => _ <- _ _ //; exact : (pos_leb_trans Hnegls1 (pos_leb_trans Hnewudiv (pos_leb_trans Hnewxorr (pos_leb_trans Hnewzextr Hnewaddr)))).
+  - dcase (mk_env_xor E_add g_add ls2 (copy (size ls2) (splitmsl ls2).2)) => [[[[E_xor2] g_xor2] cs_xor2] rs_xor2] Hmkxor2.
+    dcase (mk_env_zeroextend (size (splitmsl ls2).1) E_xor2 g_xor2 [:: (splitmsl ls2).2]) => [[[[E_zext2] g_zext2] cs_zext2] rs_zext2] Hmkzext2.
+    dcase (mk_env_add E_zext2 g_zext2 rs_xor2 rs_zext2) => [[[[E_abs2] g_abs2] cs_abs2] lrs_abs2] Hmkadd2.
+    dcase (mk_env_udiv E_abs2 g_abs2 rs_add lrs_abs2) => [[[[[E_udiv] g_udiv] cs_udiv] lqs_udiv]lrs_udiv] Hmkudiv.
+    dcase (mk_env_xor E_udiv g_udiv lrs_udiv (copy (size ls1) (splitmsl ls1).2)) => [[[[E_xorr] g_xorr] cs_xorr] rs_xorr] Hmkxorr.
+    dcase (mk_env_zeroextend (size (splitmsl ls1).1) E_xorr g_xorr [:: (splitmsl ls1).2]) => [[[[E_zextr] g_zextr] cs_zextr] rs_zextr] Hmkzextr.
+    dcase (mk_env_add E_zextr g_zextr rs_xorr rs_zextr) => [[[[E_addr] g_addr] cs_addr] rs_addr] Hmkaddr.
+    move : (mk_env_xor_newer_gen Hmkxor2) => Hnewxor2.
+    move : (mk_env_zeroextend_newer_gen Hmkzext2) => Hnewzext2.
+    move : (mk_env_add_newer_gen Hmkadd2) => Hnewadd2.
+    move : (mk_env_udiv_newer_gen Hmkudiv) => Hnewudiv.
+    move : (mk_env_xor_newer_gen Hmkxorr) => Hnewxorr.
+    move : (mk_env_zeroextend_newer_gen Hmkzextr) => Hnewzextr.
+    move : (mk_env_add_newer_gen Hmkaddr) => Hnewaddr.
+    case  => _ <- _ _ //; exact : (pos_leb_trans Hnegls1 (pos_leb_trans Hnewxor2 (pos_leb_trans Hnewzext2 (pos_leb_trans Hnewadd2 (pos_leb_trans Hnewudiv (pos_leb_trans Hnewxorr (pos_leb_trans Hnewzextr Hnewaddr))))))).
+Qed.
+
+Lemma mk_env_srem_newer_res :
+  forall ls1 E g ls2 E' g' cs lrs,
+    mk_env_srem E g ls1 ls2  = (E', g', cs, lrs) ->
+    newer_than_lit g lit_tt ->
+    newer_than_lits g ls1 ->
+    newer_than_lits g ls2 ->
+    newer_than_lits g' lrs.
+Proof.
+  rewrite /mk_env_srem /mk_env_abs.  move => ls1 E g ls2 E' g' cs rlrs.
+  dcase (mk_env_neg E g ls1) => [[[[E_neg1] g_neg1] cs_neg1] rs_neg1] Hmkneg1.
+  dcase (mk_env_xor E g ls1 (copy (size ls1) (splitmsl ls1).2)) => [[[[E_xor1] g_xor1] cs_xor1] rs_xor1] Hmkxor1.
+  dcase (mk_env_zeroextend (size (splitmsl ls1).1) E_xor1 g_xor1 [:: (splitmsl ls1).2]) => [[[[E_zext1] g_zext1] cs_zext1] rs_zext1] Hmkzext1.
+  dcase (mk_env_add E_zext1 g_zext1 rs_xor1 rs_zext1) => [[[[E_add] g_add] cs_add] rs_add] Hmkadd1.
+  move : (mk_env_neg_newer_gen Hmkneg1) => Hnewneg1.
+  move : (mk_env_xor_newer_gen Hmkxor1) => Hnewxor1.
+  move : (mk_env_zeroextend_newer_gen Hmkzext1) => Hnewzext1.
+  move : (mk_env_add_newer_gen Hmkadd1) => Hnewadd1.
+  move : (pos_leb_trans Hnewxor1 (pos_leb_trans Hnewzext1 Hnewadd1)) => Hnegls1.
+  case Htt1: ((splitmsl ls1).2 == lit_tt); case Hff1 : ((splitmsl ls1).2 == lit_ff);
+    case Htt2 : ((splitmsl ls2).2 == lit_tt); case Hff2 : ((splitmsl ls2).2 == lit_ff);
+      try rewrite (eqP Htt1)// in Hff1; try rewrite (eqP Htt2)// in Hff2.
+  - dcase (mk_env_neg E_neg1 g_neg1 ls2) => [[[[E_abs2] g_abs2] cs_abs2] lrs_abs2] Hmkneg2.
+    dcase (mk_env_udiv E_abs2 g_abs2 rs_neg1 lrs_abs2) => [[[[[E_udiv] g_udiv] cs_udiv] lqs_udiv]lrs_udiv] Hmkudiv.
+    dcase (mk_env_neg E_udiv g_udiv lrs_udiv) => [[[[E_negr] g_negr] cs_negr] lrs_negr] Hmknegr.
+    move : (mk_env_neg_newer_gen Hmkneg2) => Hnewneg2.
+    move : (mk_env_udiv_newer_gen Hmkudiv) => Hnewudiv.
+    case => _ <- _ <- //; move => Htt Hls1 Hls2.
+    move : (mk_env_neg_newer_res Hmkneg1 Htt Hls1) => Hgneg1.
+    move : (mk_env_neg_newer_res Hmkneg2 (newer_than_lit_le_newer Htt Hnewneg1) (newer_than_lits_le_newer Hls2 Hnewneg1)) => Hgneg2.
+    move/andP : (mk_env_udiv_newer_res Hmkudiv (newer_than_lit_le_newer Htt (pos_leb_trans Hnewneg1 Hnewneg2)) (newer_than_lits_le_newer Hgneg1 Hnewneg2) Hgneg2) => [Hgudiv _].
+    exact : (mk_env_neg_newer_res Hmknegr (newer_than_lit_le_newer Htt (pos_leb_trans Hnewneg1 (pos_leb_trans Hnewneg2 Hnewudiv))) Hgudiv) => Hgnegr.
+  - dcase (mk_env_udiv E_neg1 g_neg1 rs_neg1 ls2) => [[[[[E_udiv] g_udiv] cs_udiv] lqs_udiv]lrs_udiv] Hmkudiv.
+    dcase (mk_env_neg E_udiv g_udiv lrs_udiv) => [[[[E_negr] g_negr] cs_negr] lrs_negr] Hmknegr.
+    move : (mk_env_udiv_newer_gen Hmkudiv) => Hnewudiv.
+    case => _ <- _ <- //; move => Htt Hls1 Hls2.
+    move : (mk_env_neg_newer_res Hmkneg1 Htt Hls1) => Hgneg1.
+    move/andP : (mk_env_udiv_newer_res Hmkudiv (newer_than_lit_le_newer Htt Hnewneg1) Hgneg1 (newer_than_lits_le_newer Hls2 Hnewneg1)) => [Hgudiv _].
+    exact : (mk_env_neg_newer_res Hmknegr (newer_than_lit_le_newer Htt (pos_leb_trans Hnewneg1 Hnewudiv)) Hgudiv).
+  - dcase (mk_env_xor E_neg1 g_neg1 ls2 (copy (size ls2) (splitmsl ls2).2)) => [[[[E_xor2] g_xor2] cs_xor2] rs_xor2] Hmkxor2.
+    dcase (mk_env_zeroextend (size (splitmsl ls2).1) E_xor2 g_xor2 [:: (splitmsl ls2).2]) => [[[[E_zext2] g_zext2] cs_zext2] rs_zext2] Hmkzext2.
+    dcase (mk_env_add E_zext2 g_zext2 rs_xor2 rs_zext2) => [[[[E_add2] g_add2] cs_add2] rs_add2] Hmkadd2.
+    dcase (mk_env_udiv E_add2 g_add2 rs_neg1 rs_add2) => [[[[[E_udiv] g_udiv] cs_udiv] lqs_udiv] lrs_udiv] Hmkudiv.
+    dcase (mk_env_neg E_udiv g_udiv lrs_udiv) => [[[[E_negr] g_negr] cs_negr] lrs_negr] Hmknegr.
+    move : (mk_env_xor_newer_gen Hmkxor2) => Hnewxor2.
+    move : (mk_env_zeroextend_newer_gen Hmkzext2) => Hnewzext2.
+    move : (mk_env_add_newer_gen Hmkadd2) => Hnewadd2.
+    move : (mk_env_udiv_newer_gen Hmkudiv) => Hnewudiv.
+    case => _ <- _ <- //; move => Htt Hls1 Hls2.
+    move : (mk_env_neg_newer_res Hmkneg1 Htt Hls1) => Hgneg1.
+    move : (mk_env_add_newer_res Hmkadd2) => Hgneg2.
+    move/andP : (mk_env_udiv_newer_res Hmkudiv (newer_than_lit_le_newer Htt (pos_leb_trans Hnewneg1 (pos_leb_trans Hnewxor2 (pos_leb_trans Hnewzext2 Hnewadd2)))) (newer_than_lits_le_newer Hgneg1 (pos_leb_trans Hnewxor2 (pos_leb_trans Hnewzext2 Hnewadd2))) Hgneg2) => [Hgudiv _].
+    exact : (mk_env_neg_newer_res Hmknegr (newer_than_lit_le_newer Htt (pos_leb_trans Hnewneg1 (pos_leb_trans Hnewxor2 (pos_leb_trans Hnewzext2 (pos_leb_trans Hnewadd2 Hnewudiv))))) Hgudiv).
+  - dcase (mk_env_neg E g ls2) => [[[[E_abs2] g_abs2] cs_abs2] lrs_abs2] Hmkneg2.
+    dcase (mk_env_udiv E_abs2 g_abs2 ls1 lrs_abs2) => [[[[[E_udiv] g_udiv] cs_udiv] lqs_udiv]lrs_udiv] Hmkudiv.
+    move : (mk_env_neg_newer_gen Hmkneg2) => Hnewneg2.
+    case => _ <- _ <- //; move => Htt Hls1 Hls2.
+    move : (mk_env_neg_newer_res Hmkneg2 Htt Hls2) => Hgneg2.
+    move/andP : (mk_env_udiv_newer_res Hmkudiv (newer_than_lit_le_newer Htt Hnewneg2) (newer_than_lits_le_newer Hls1 Hnewneg2) Hgneg2) => [Hgudiv _]; done.
+  - dcase (mk_env_udiv E g ls1 ls2) => [[[[[E_udiv] g_udiv] cs_udiv] lqs_udiv]lrs_udiv] Hmkudiv.
+    case => _ <- _ <- //; move => Htt Hls1 Hls2.
+    move/andP : (mk_env_udiv_newer_res Hmkudiv Htt Hls1 Hls2) => [Hgudiv _]; done. 
+  - dcase (mk_env_xor E g ls2 (copy (size ls2) (splitmsl ls2).2)) => [[[[E_xor2] g_xor2] cs_xor2] rs_xor2] Hmkxor2.
+    dcase (mk_env_zeroextend (size (splitmsl ls2).1) E_xor2 g_xor2 [:: (splitmsl ls2).2]) => [[[[E_zext2] g_zext2] cs_zext2] rs_zext2] Hmkzext2.
+    dcase (mk_env_add E_zext2 g_zext2 rs_xor2 rs_zext2) => [[[[E_add2] g_add2] cs_add2] rs_add2] Hmkadd2.
+    dcase (mk_env_udiv E_add2 g_add2 ls1 rs_add2) => [[[[[E_udiv] g_udiv] cs_udiv] lqs_udiv] lrs_udiv] Hmkudiv.
+    move : (mk_env_xor_newer_gen Hmkxor2) => Hnewxor2.
+    move : (mk_env_zeroextend_newer_gen Hmkzext2) => Hnewzext2.
+    move : (mk_env_add_newer_gen Hmkadd2) => Hnewadd2.
+    case => _ <- _ <- //; move => Htt Hls1 Hls2.
+    move : (pos_leb_trans Hnewxor2 (pos_leb_trans Hnewzext2 Hnewadd2)) => Hggadd2.
+    move : (mk_env_add_newer_res Hmkadd2) => Hgadd2.
+    move/andP : (mk_env_udiv_newer_res Hmkudiv (newer_than_lit_le_newer Htt Hggadd2) (newer_than_lits_le_newer Hls1 Hggadd2) Hgadd2) => [Hgudiv _]; done.
+  - dcase (mk_env_neg E_add g_add ls2) => [[[[E_abs2] g_abs2] cs_abs2] lrs_abs2] Hmkneg2.
+    dcase (mk_env_udiv E_abs2 g_abs2 rs_add lrs_abs2) => [[[[[E_udiv] g_udiv] cs_udiv] lqs_udiv]lrs_udiv] Hmkudiv.
+    dcase (mk_env_xor E_udiv g_udiv lrs_udiv (copy (size ls1) (splitmsl ls1).2)) => [[[[E_xorr] g_xorr] cs_xorr] rs_xorr] Hmkxorr.
+    dcase (mk_env_zeroextend (size (splitmsl ls1).1) E_xorr g_xorr [:: (splitmsl ls1).2]) => [[[[E_zextr] g_zextr] cs_zextr] rs_zextr] Hmkzextr.
+    dcase (mk_env_add E_zextr g_zextr rs_xorr rs_zextr) => [[[[E_addr] g_addr] cs_addr] rs_addr] Hmkaddr.
+    case => _ <- _ <- //; move => Htt Hls1 Hls2.
+    exact : (mk_env_add_newer_res Hmkaddr).
+  - dcase (mk_env_udiv E_add g_add rs_add ls2) => [[[[[E_udiv] g_udiv] cs_udiv] lqs_udiv]lrs_udiv] Hmkudiv.
+    dcase (mk_env_xor E_udiv g_udiv lrs_udiv (copy (size ls1) (splitmsl ls1).2)) => [[[[E_xorr] g_xorr] cs_xorr] rs_xorr] Hmkxorr.
+    dcase (mk_env_zeroextend (size (splitmsl ls1).1) E_xorr g_xorr [:: (splitmsl ls1).2]) => [[[[E_zextr] g_zextr] cs_zextr] rs_zextr] Hmkzextr.
+    dcase (mk_env_add E_zextr g_zextr rs_xorr rs_zextr) => [[[[E_addr] g_addr] cs_addr] rs_addr] Hmkaddr.
+    case => _ <- _ <- //; move => Htt Hls1 Hls2.
+    exact : (mk_env_add_newer_res Hmkaddr).
+  - dcase (mk_env_xor E_add g_add ls2 (copy (size ls2) (splitmsl ls2).2)) => [[[[E_xor2] g_xor2] cs_xor2] rs_xor2] Hmkxor2.
+    dcase (mk_env_zeroextend (size (splitmsl ls2).1) E_xor2 g_xor2 [:: (splitmsl ls2).2]) => [[[[E_zext2] g_zext2] cs_zext2] rs_zext2] Hmkzext2.
+    dcase (mk_env_add E_zext2 g_zext2 rs_xor2 rs_zext2) => [[[[E_abs2] g_abs2] cs_abs2] lrs_abs2] Hmkadd2.
+    dcase (mk_env_udiv E_abs2 g_abs2 rs_add lrs_abs2) => [[[[[E_udiv] g_udiv] cs_udiv] lqs_udiv]lrs_udiv] Hmkudiv.
+    dcase (mk_env_xor E_udiv g_udiv lrs_udiv (copy (size ls1) (splitmsl ls1).2)) => [[[[E_xorr] g_xorr] cs_xorr] rs_xorr] Hmkxorr.
+    dcase (mk_env_zeroextend (size (splitmsl ls1).1) E_xorr g_xorr [:: (splitmsl ls1).2]) => [[[[E_zextr] g_zextr] cs_zextr] rs_zextr] Hmkzextr.
+    dcase (mk_env_add E_zextr g_zextr rs_xorr rs_zextr) => [[[[E_addr] g_addr] cs_addr] rs_addr] Hmkaddr.
+    case => _ <- _ <- //; move => Htt Hls1 Hls2.
+    exact : (mk_env_add_newer_res Hmkaddr).
+Qed.
+
+
+Lemma mk_env_abs_newer_gen :
+  forall E g ls E' g' cs lrs,
+    mk_env_abs E g ls = (E', g', cs, lrs) ->
+    (g <=? g')%positive.
+Proof.
+  move=> E g ls E' g' cs lrs. rewrite /mk_env_abs.
+  case ((splitmsl ls).2 == lit_tt); last case ((splitmsl ls).2 == lit_ff).
+  - exact: mk_env_neg_newer_gen.
+  - case=> _ <- _ _. by rewrite Pos.leb_refl.
+  - dcase (mk_env_xor E g ls (copy (size ls) (splitmsl ls).2)) 
+    => [[[[E_xor] g_xor] cs_xor] lrs_xor] Hmkxor.
+    dcase (mk_env_zeroextend (size (splitmsl ls).1) E_xor g_xor [:: (splitmsl ls).2])
+    => [[[[E_zext] g_zext] cs_zext] lrs_zext] Hmkzext.
+    dcase (mk_env_add E_zext g_zext lrs_xor lrs_zext)
+    => [[[[E_add] g_add] cs_add] lrs_add] Hmkadd.
+    case=> _ <- _ _.
+    move: (mk_env_xor_newer_gen Hmkxor) => Hggxor.
+    move: (mk_env_zeroextend_newer_gen Hmkzext) => Hgxorgzext.
+    move: (mk_env_add_newer_gen Hmkadd) => Hgzextgadd.
+    by apply (pos_leb_trans Hggxor); apply (pos_leb_trans Hgxorgzext).
+Qed.
+
+Lemma mk_env_abs_newer_res :
+  forall E g ls E' g' cs lrs,
+    mk_env_abs E g ls = (E', g', cs, lrs) ->
+    newer_than_lit g lit_tt ->
+    newer_than_lits g ls ->
+    newer_than_lits g' lrs.
+Proof.
+  move=> E g ls E' g' cs lrs. rewrite /mk_env_abs.
+  case ((splitmsl ls).2 == lit_tt); last case ((splitmsl ls).2 == lit_ff).
+  - exact: mk_env_neg_newer_res.
+  - by case=> _ <- _ <-. 
+  - dcase (mk_env_xor E g ls (copy (size ls) (splitmsl ls).2)) 
+    => [[[[E_xor] g_xor] cs_xor] lrs_xor] Hmkxor.
+    dcase (mk_env_zeroextend (size (splitmsl ls).1) E_xor g_xor [:: (splitmsl ls).2])
+    => [[[[E_zext] g_zext] cs_zext] lrs_zext] Hmkzext.
+    dcase (mk_env_add E_zext g_zext lrs_xor lrs_zext)
+    => [[[[E_add] g_add] cs_add] lrs_add] Hmkadd.
+    case=> _ <- _ <- Hgtt Hgls.
+    exact: (mk_env_add_newer_res Hmkadd).
+Qed.
+
+Lemma mk_env_abs_newer_cnf :
+  forall E g ls E' g' cs lrs,
+    mk_env_abs E g ls = (E', g', cs, lrs) ->
+    newer_than_lit g lit_tt ->
+    newer_than_lits g ls ->
+    newer_than_cnf g' cs.
+Proof.
+  move=> E g ls E' g' cs lrs. rewrite /mk_env_abs.
+  case ((splitmsl ls).2 == lit_tt); last case ((splitmsl ls).2 == lit_ff).
+  - exact: mk_env_neg_newer_cnf.
+  - by case=> _ <- <- _. 
+  - dcase (mk_env_xor E g ls (copy (size ls) (splitmsl ls).2)) 
+    => [[[[E_xor] g_xor] cs_xor] lrs_xor] Hmkxor.
+    dcase (mk_env_zeroextend (size (splitmsl ls).1) E_xor g_xor [:: (splitmsl ls).2])
+    => [[[[E_zext] g_zext] cs_zext] lrs_zext] Hmkzext.
+    dcase (mk_env_add E_zext g_zext lrs_xor lrs_zext)
+    => [[[[E_add] g_add] cs_add] lrs_add] Hmkadd.
+    case=> _ <- <- _ Hgtt Hgls.
+    move: (mk_env_xor_newer_gen Hmkxor) => Hggxor.
+    move: (mk_env_zeroextend_newer_gen Hmkzext) => Hgxorgzext.
+    move: (mk_env_add_newer_gen Hmkadd) => Hgzextgadd.
+    move: (newer_than_lits_msl Hgtt Hgls) => Hgmsl.
+    move: (newer_than_lits_copy (size ls) Hgmsl) => Hgcopy.
+    move: (mk_env_xor_newer_cnf Hmkxor Hgtt Hgls Hgcopy) => Hgxorcsxor.
+    move: (newer_than_cnf_le_newer Hgxorcsxor (pos_leb_trans Hgxorgzext Hgzextgadd)) => Hgaddcsxor.
+    move: (newer_than_lit_le_newer Hgtt Hggxor) => Hgxortt.
+    move: (newer_than_lit_le_newer Hgmsl Hggxor) => Hgxormsl.
+    move: (newer_than_lits_copy 1 Hgxormsl) => Hgxor1msl.
+    move: (mk_env_zeroextend_newer_cnf Hmkzext Hgxortt Hgxor1msl) => Hgzextcszext.
+    move: (newer_than_cnf_le_newer Hgzextcszext Hgzextgadd) => Hgaddcszext.
+    move: (mk_env_xor_newer_res Hmkxor Hgtt Hgls Hgcopy) => Hgxorlxor.
+    move: (newer_than_lits_le_newer Hgxorlxor Hgxorgzext) => Hgzextlxor.
+    move: (mk_env_zeroextend_newer_res Hmkzext Hgxortt Hgxor1msl) => Hgzextlzext.
+    move: (newer_than_lit_le_newer Hgxortt Hgxorgzext) => Hgzexttt.
+    rewrite newer_than_lit_tt_ff in Hgzexttt.
+    move: (mk_env_add_newer_cnf Hmkadd Hgzextlxor Hgzextlzext Hgzexttt) => Hgaddcsadd.
+    by rewrite !newer_than_cnf_catrev Hgaddcsxor Hgaddcszext Hgaddcsadd.
+Qed.
+
+Lemma mk_env_abs_preserve :
+  forall E g ls E' g' cs lrs,
+    mk_env_abs E g ls = (E', g', cs, lrs) ->
+    env_preserve E E' g.
+Proof.
+  move=> E g ls E' g' cs lrs. rewrite /mk_env_abs.
+  case ((splitmsl ls).2 == lit_tt); last case ((splitmsl ls).2 == lit_ff).
+  - exact: mk_env_neg_preserve.
+  - by case=> <- _ _ _. 
+  - dcase (mk_env_xor E g ls (copy (size ls) (splitmsl ls).2)) 
+    => [[[[E_xor] g_xor] cs_xor] lrs_xor] Hmkxor.
+    dcase (mk_env_zeroextend (size (splitmsl ls).1) E_xor g_xor [:: (splitmsl ls).2])
+    => [[[[E_zext] g_zext] cs_zext] lrs_zext] Hmkzext.
+    dcase (mk_env_add E_zext g_zext lrs_xor lrs_zext)
+    => [[[[E_add] g_add] cs_add] lrs_add] Hmkadd.
+    case=> <- _ _ _. 
+    move: (mk_env_xor_newer_gen Hmkxor) => Hggxor.
+    move: (mk_env_zeroextend_newer_gen Hmkzext) => Hgxorgzext.
+    move: (mk_env_add_newer_gen Hmkadd) => Hgzextgadd.
+    move: (mk_env_xor_preserve Hmkxor) => HEExorg.
+    move: (mk_env_zeroextend_preserve Hmkzext) => HExorEzextgxor.
+    move: (mk_env_add_preserve Hmkadd) => HEzextEaddgzext. 
+    move: (env_preserve_le HExorEzextgxor Hggxor) => HExorEzextg.
+    move: (env_preserve_le HEzextEaddgzext (pos_leb_trans Hggxor Hgxorgzext)) => HEzextEaddg.
+    by apply (env_preserve_trans HEExorg); apply (env_preserve_trans HExorEzextg).
+Qed.    
+
+Lemma mk_env_srem_newer_cnf :
+  forall ls1 E g ls2 E' g' cs lrs,
+    mk_env_srem E g ls1 ls2 = (E', g', cs, lrs) ->
+    newer_than_lit g lit_tt ->
+    newer_than_lits g ls1 ->
+    newer_than_lits g ls2 ->
+    newer_than_cnf g' cs.
+Proof.
+  move=> ls1 E g ls2 E' g' cs lrs. rewrite /mk_env_srem.
+  dcase (mk_env_abs E g ls1) => [[[[E_abs1] g_abs1] cs_abs1] lrs_abs1] Hmkabs1.
+  dcase (mk_env_abs E_abs1 g_abs1 ls2) => [[[[E_abs2] g_abs2] cs_abs2] lrs_abs2] Hmkabs2.
+  dcase (mk_env_udiv E_abs2 g_abs2 lrs_abs1 lrs_abs2) => [[[[[E_udiv] g_udiv] cs_udiv] lrs_udiv] lrs_urem] Hmkudiv.
+  move=> H Hgtt Hgls1 Hgls2; move: H.
+  move: (mk_env_abs_newer_gen Hmkabs1) => Hggabs1.
+  move: (mk_env_abs_newer_gen Hmkabs2) => Hgabs1gabs2.
+  move: (mk_env_udiv_newer_gen Hmkudiv) => Hgabs2gudiv.
+  move: (mk_env_abs_newer_cnf Hmkabs1 Hgtt Hgls1) => Hgabs1csabs1.
+  move: (newer_than_cnf_le_newer Hgabs1csabs1 (pos_leb_trans Hgabs1gabs2 Hgabs2gudiv)) => Hgudivcsabs1.
+  move: (newer_than_lit_le_newer Hgtt Hggabs1) => Hgabs1tt.
+  move: (newer_than_lits_le_newer Hgls2 Hggabs1) => Hgabs1ls2.
+  move: (mk_env_abs_newer_cnf Hmkabs2 Hgabs1tt Hgabs1ls2) => Hgabs2csabs2.
+  move: (newer_than_cnf_le_newer Hgabs2csabs2 Hgabs2gudiv) => Hgudivcsabs2.
+  move: (newer_than_lit_le_newer Hgabs1tt Hgabs1gabs2) => Hgabs2tt.
+  move: (mk_env_abs_newer_res Hmkabs1 Hgtt Hgls1) => Hgabs1labs1.
+  move: (newer_than_lits_le_newer Hgabs1labs1 Hgabs1gabs2) => Hgabs2labs1.
+  move: (mk_env_abs_newer_res Hmkabs2 Hgabs1tt Hgabs1ls2) => Hgabs2labs2.
+  move: (mk_env_udiv_newer_cnf Hmkudiv Hgabs2tt Hgabs2labs1 Hgabs2labs2) => Hgudivcsudiv.
+  case ((splitmsl ls1).2 == lit_ff); last case ((splitmsl ls1).2 == lit_tt).
+  - case=> _ <- <- _.
+    by rewrite !newer_than_cnf_catrev Hgudivcsabs1 Hgudivcsabs2 Hgudivcsudiv.
+  - dcase (mk_env_neg E_udiv g_udiv lrs_urem) => [[[[E_neg] g_neg] cs_neg] lrs_neg] Hmkneg.
+    case=> _ <- <- _.
+    move: (mk_env_neg_newer_gen Hmkneg) => Hgudivgneg.
+    move: (newer_than_cnf_le_newer Hgudivcsabs1 Hgudivgneg) => Hgnegcsabs1.
+    move: (newer_than_cnf_le_newer Hgudivcsabs2 Hgudivgneg) => Hgnegcsabs2.
+    move: (newer_than_cnf_le_newer Hgudivcsudiv Hgudivgneg) => Hgnegcsudiv.
+    move: (newer_than_lit_le_newer Hgabs2tt Hgabs2gudiv) => Hgudivtt.
+    move: (mk_env_udiv_newer_res Hmkudiv Hgabs2tt Hgabs2labs1 Hgabs2labs2) => /andP [Hgudivlurem _].
+    move: (mk_env_neg_newer_cnf Hmkneg Hgudivtt Hgudivlurem) => Hgnegcsneg.
+    by rewrite !newer_than_cnf_catrev Hgnegcsabs1 Hgnegcsabs2 Hgnegcsudiv Hgnegcsneg.
+  - dcase (mk_env_xor E_udiv g_udiv lrs_urem (copy (size ls1) (splitmsl ls1).2)) 
+    => [[[[E_xor] g_xor] cs_xor] lrs_xor] Hmkxor.
+    dcase (mk_env_zeroextend (size (splitmsl ls1).1) E_xor g_xor [::(splitmsl ls1).2])
+    => [[[[E_zext] g_zext] cs_zext] lrs_zext] Hmkzext.
+    dcase (mk_env_add E_zext g_zext lrs_xor lrs_zext)
+    => [[[[E_add] g_add] cs_add] lrs_add] Hmkadd.
+    case=> _ <- <- _.
+    move: (mk_env_xor_newer_gen Hmkxor) => Hgudivgxor.
+    move: (mk_env_zeroextend_newer_gen Hmkzext) => Hgxorgzext.
+    move: (mk_env_add_newer_gen Hmkadd) => Hgzextgadd.
+    move: (pos_leb_trans Hgudivgxor (pos_leb_trans Hgxorgzext Hgzextgadd)) => Hgudivgadd.
+    move: (newer_than_cnf_le_newer Hgudivcsabs1 Hgudivgadd) => Hgaddcsabs1.
+    move: (newer_than_cnf_le_newer Hgudivcsabs2 Hgudivgadd) => Hgaddcsabs2.
+    move: (newer_than_cnf_le_newer Hgudivcsudiv Hgudivgadd) => Hgaddcsudiv.
+    move: (newer_than_lit_le_newer Hgabs2tt Hgabs2gudiv) => Hgudivtt.
+    move: (mk_env_udiv_newer_res Hmkudiv Hgabs2tt Hgabs2labs1 Hgabs2labs2) => /andP [Hgudivlurem _].
+    move: (newer_than_lits_le_newer Hgls1 (pos_leb_trans Hggabs1 (pos_leb_trans Hgabs1gabs2 Hgabs2gudiv))) => Hgudivls1.
+    move: (newer_than_lits_msl Hgudivtt Hgudivls1) => Hgudivmsl1.
+    move: (newer_than_lits_copy (size ls1) Hgudivmsl1) => Hgudivcopy.
+    move: (mk_env_xor_newer_cnf Hmkxor Hgudivtt Hgudivlurem Hgudivcopy) => Hgxorcsxor.
+    move: (newer_than_cnf_le_newer Hgxorcsxor (pos_leb_trans Hgxorgzext Hgzextgadd)) => Hgaddcsxor.
+    move: (newer_than_lit_le_newer Hgudivtt Hgudivgxor) => Hgxortt.
+    move: (newer_than_lit_le_newer Hgudivmsl1 Hgudivgxor) => Hgxormsl1.
+    move: (newer_than_lits_copy 1 Hgxormsl1) => Hgxor1msl1.
+    move: (mk_env_zeroextend_newer_cnf Hmkzext Hgxortt Hgxor1msl1) => Hgzextcszext.
+    move: (newer_than_cnf_le_newer Hgzextcszext Hgzextgadd) => Hgaddcszext.
+    move: (mk_env_xor_newer_res Hmkxor Hgudivtt Hgudivlurem Hgudivcopy) => Hgxorlxor.
+    move: (newer_than_lits_le_newer Hgxorlxor Hgxorgzext) => Hgzextlxor.
+    move: (mk_env_zeroextend_newer_res Hmkzext Hgxortt Hgxor1msl1) => Hgzextlzext.
+    move: (newer_than_lit_le_newer Hgxortt Hgxorgzext) => Hgzexttt.
+    rewrite newer_than_lit_tt_ff in Hgzexttt.
+    move: (mk_env_add_newer_cnf Hmkadd Hgzextlxor Hgzextlzext Hgzexttt) => Hgaddcsadd.
+    by rewrite !newer_than_cnf_catrev Hgaddcsabs1 Hgaddcsabs2 Hgaddcsudiv 
+               Hgaddcsxor Hgaddcszext Hgaddcsadd.
+Qed.
+
+Lemma mk_env_srem_preserve :
+  forall E g ls1 ls2 E' g' cs lrs,
+    mk_env_srem E g ls1 ls2 = (E', g', cs, lrs) ->
+    env_preserve E E' g.
+Proof.
+  move=> E g ls1 ls2 E' g' cs lrs. rewrite /mk_env_srem.
+  dcase (mk_env_abs E g ls1) => [[[[E_abs1] g_abs1] cs_abs1] lrs_abs1] Hmkabs1.
+  dcase (mk_env_abs E_abs1 g_abs1 ls2) => [[[[E_abs2] g_abs2] cs_abs2] lrs_abs2] Hmkabs2.
+  dcase (mk_env_udiv E_abs2 g_abs2 lrs_abs1 lrs_abs2) => [[[[[E_udiv] g_udiv] cs_udiv] lrs_udiv] lrs_urem] Hmkudiv.
+  move: (mk_env_abs_newer_gen Hmkabs1) => Hggabs1.
+  move: (mk_env_abs_newer_gen Hmkabs2) => Hgabs1gabs2.
+  move: (mk_env_udiv_newer_gen Hmkudiv) => Hgabs2gudiv.
+  move: (mk_env_abs_preserve Hmkabs1) => HEEabs1g.
+  move: (mk_env_abs_preserve Hmkabs2) => HEabs1Eabs2gabs1.
+  move: (env_preserve_le HEabs1Eabs2gabs1 Hggabs1) => HEabs1Eabs2g.
+  move: (mk_env_udiv_preserve Hmkudiv) => HEabs2Eudivgabs2.
+  move: (env_preserve_le HEabs2Eudivgabs2 (pos_leb_trans Hggabs1 Hgabs1gabs2)) => HEabs2Eudivg.
+  case ((splitmsl ls1).2 == lit_ff); last case ((splitmsl ls1).2 == lit_tt).
+  - case=> <- _ _ _. by t_auto_preserve.
+  - dcase (mk_env_neg E_udiv g_udiv lrs_urem) 
+    => [[[[E_neg] g_neg] cs_neg] lrs_neg] Hmkneg.
+    case=> <- _ _ _.
+    move: (mk_env_neg_newer_gen Hmkneg) => Hgudivgneg.
+    move: (mk_env_neg_preserve Hmkneg) => HEudivEneggudiv.
+    by t_auto_preserve.
+  - dcase (mk_env_xor E_udiv g_udiv lrs_urem (copy (size ls1) (splitmsl ls1).2)) 
+    => [[[[E_xor] g_xor] cs_xor] lrs_xor] Hmkxor.
+    dcase (mk_env_zeroextend (size (splitmsl ls1).1) E_xor g_xor [::(splitmsl ls1).2])
+    => [[[[E_zext] g_zext] cs_zext] lrs_zext] Hmkzext.
+    dcase (mk_env_add E_zext g_zext lrs_xor lrs_zext)
+    => [[[[E_add] g_add] cs_add] lrs_add] Hmkadd.
+    case=> <- _ _ _.
+    move: (mk_env_xor_newer_gen Hmkxor) => Hgudivgxor.
+    move: (mk_env_zeroextend_newer_gen Hmkzext) => Hgxorgzext.
+    move: (mk_env_add_newer_gen Hmkadd) => Hgzextgadd.
+    move: (mk_env_xor_preserve Hmkxor) => HEudivExorgudiv.
+    move: (mk_env_zeroextend_preserve Hmkzext) => HExorEzextgxor.
+    move: (mk_env_add_preserve Hmkadd) => HEzextEaddgzext.
+    move: (env_preserve_le HExorEzextgxor Hgudivgxor) => HExorEzextgudiv.
+    move: (env_preserve_le HEzextEaddgzext (pos_leb_trans Hgudivgxor Hgxorgzext)) => HEzextEaddgudiv.
+    move: (pos_leb_trans Hggabs1 (pos_leb_trans Hgabs1gabs2 Hgabs2gudiv)) => Hggudiv.
+    move: (env_preserve_le HEudivExorgudiv Hggudiv) => HEudivExorg.
+    move: (env_preserve_le HExorEzextgudiv Hggudiv) => HExorEzextg.
+    move: (env_preserve_le HEzextEaddgudiv Hggudiv) => HEzextEaddg.
+    apply (env_preserve_trans HEEabs1g); apply (env_preserve_trans HEabs1Eabs2g);
+    apply (env_preserve_trans HEabs2Eudivg); apply (env_preserve_trans HEudivExorg);
+    by apply (env_preserve_trans HExorEzextg).
+Qed.
+
+Lemma mk_env_srem_sat :
+  forall E g ls1 ls2 E' g' cs lrs,
+    mk_env_srem E g ls1 ls2 = (E', g', cs, lrs) ->
+    newer_than_lit g lit_tt ->
+    newer_than_lits g ls1 ->
+    newer_than_lits g ls2 ->
+    interp_cnf E' cs.
+Proof.
+  move => E g ls1 ls2 E' g' cs lrs. rewrite /mk_env_srem /mk_env_abs.
+  dcase (mk_env_neg E g ls1) => [[[[E_neg1] g_neg1] cs_neg1] rs_neg1] Hmkneg1.
+  dcase (mk_env_xor E g ls1 (copy (size ls1) (splitmsl ls1).2)) => [[[[E_xor1] g_xor1] cs_xor1] rs_xor1] Hmkxor1.
+  dcase (mk_env_zeroextend (size (splitmsl ls1).1) E_xor1 g_xor1 [:: (splitmsl ls1).2]) => [[[[E_zext1] g_zext1] cs_zext1] rs_zext1] Hmkzext1.
+  dcase (mk_env_add E_zext1 g_zext1 rs_xor1 rs_zext1) => [[[[E_add] g_add] cs_add] rs_add] Hmkadd1.
+  move : (mk_env_neg_newer_gen Hmkneg1) => Hnewneg1.
+  move : (mk_env_xor_newer_gen Hmkxor1) => Hnewxor1.
+  move : (mk_env_zeroextend_newer_gen Hmkzext1) => Hnewzext1.
+  move : (mk_env_add_newer_gen Hmkadd1) => Hnewadd1.
+  move : (pos_leb_trans Hnewxor1 (pos_leb_trans Hnewzext1 Hnewadd1)) => Hnegls1.
+  case Htt1: ((splitmsl ls1).2 == lit_tt); case Hff1 : ((splitmsl ls1).2 == lit_ff);
+    case Htt2 : ((splitmsl ls2).2 == lit_tt); case Hff2 : ((splitmsl ls2).2 == lit_ff);
+      try rewrite (eqP Htt1)// in Hff1; try rewrite (eqP Htt2)// in Hff2.
+  - dcase (mk_env_neg E_neg1 g_neg1 ls2) => [[[[E_abs2] g_abs2] cs_abs2] lrs_abs2] Hmkneg2.
+    dcase (mk_env_udiv E_abs2 g_abs2 rs_neg1 lrs_abs2) => [[[[[E_udiv] g_udiv] cs_udiv] lqs_udiv]lrs_udiv] Hmkudiv.
+    dcase (mk_env_neg E_udiv g_udiv lrs_udiv) => [[[[E_negr] g_negr] cs_negr] lrs_negr] Hmknegr.
+    move : (mk_env_neg_newer_gen Hmkneg2) => Hnewneg2.
+    move : (mk_env_udiv_newer_gen Hmkudiv) => Hnewudiv.
+    case => <- _ <- _ //; move => Htt Hls1 Hls2; generalize Htt; rewrite newer_than_lit_tt_ff; move => Hff.
+    move : (mk_env_neg_newer_res Hmkneg1 Htt Hls1) => Hgneg1.
+    move : (mk_env_neg_newer_res Hmkneg2 (newer_than_lit_le_newer Htt Hnewneg1) (newer_than_lits_le_newer Hls2 Hnewneg1)) => Hgneg2.
+    move/andP : (mk_env_udiv_newer_res Hmkudiv (newer_than_lit_le_newer Htt (pos_leb_trans Hnewneg1 Hnewneg2)) (newer_than_lits_le_newer Hgneg1 Hnewneg2) Hgneg2) => [Hgudiv _].
+    move : (mk_env_neg_sat Hmkneg1 Hff Hls1) => Hcnfneg1.
+    move : (mk_env_neg_sat Hmkneg2 (newer_than_lit_le_newer Hff Hnewneg1) (newer_than_lits_le_newer Hls2 Hnewneg1)) => Hcnfneg2.
+    move : (mk_env_udiv_sat Hmkudiv (newer_than_lit_le_newer Htt (pos_leb_trans Hnewneg1 Hnewneg2)) (newer_than_lits_le_newer Hgneg1 Hnewneg2) Hgneg2) => Hcnfudiv.
+    move : (mk_env_neg_sat Hmknegr (newer_than_lit_le_newer Hff (pos_leb_trans Hnewneg1 (pos_leb_trans Hnewneg2 Hnewudiv))) Hgudiv) => Hcnfnegr.
+    rewrite !interp_cnf_catrev.
+    move : (mk_env_udiv_newer_cnf Hmkudiv (newer_than_lit_le_newer Htt (pos_leb_trans Hnewneg1 Hnewneg2)) (newer_than_lits_le_newer Hgneg1 Hnewneg2) Hgneg2) => Hcsudiv.
+    rewrite Hcnfnegr.
+    rewrite (env_preserve_cnf (mk_env_neg_preserve Hmknegr) (mk_env_udiv_newer_cnf Hmkudiv (newer_than_lit_le_newer Htt (pos_leb_trans Hnewneg1 Hnewneg2)) (newer_than_lits_le_newer Hgneg1 Hnewneg2) Hgneg2)) Hcnfudiv.
+    rewrite (env_preserve_cnf (mk_env_neg_preserve Hmknegr) (newer_than_cnf_le_newer (mk_env_neg_newer_cnf Hmkneg2 (newer_than_lit_le_newer Htt Hnewneg1) (newer_than_lits_le_newer Hls2 Hnewneg1)) Hnewudiv)).
+    rewrite (env_preserve_cnf (mk_env_udiv_preserve Hmkudiv) (mk_env_neg_newer_cnf Hmkneg2 (newer_than_lit_le_newer Htt Hnewneg1) (newer_than_lits_le_newer Hls2 Hnewneg1))) Hcnfneg2. 
+    rewrite (env_preserve_cnf (mk_env_neg_preserve Hmknegr) (newer_than_cnf_le_newer (mk_env_neg_newer_cnf Hmkneg1 Htt Hls1) (pos_leb_trans Hnewneg2 Hnewudiv))).
+    rewrite (env_preserve_cnf (mk_env_udiv_preserve Hmkudiv) (newer_than_cnf_le_newer (mk_env_neg_newer_cnf Hmkneg1 Htt Hls1) Hnewneg2)).
+    rewrite (env_preserve_cnf (mk_env_neg_preserve Hmkneg2) (mk_env_neg_newer_cnf Hmkneg1 Htt Hls1)) Hcnfneg1//.
+  - dcase (mk_env_udiv E_neg1 g_neg1 rs_neg1 ls2) => [[[[[E_udiv] g_udiv] cs_udiv] lqs_udiv]lrs_udiv] Hmkudiv.
+    dcase (mk_env_neg E_udiv g_udiv lrs_udiv) => [[[[E_negr] g_negr] cs_negr] lrs_negr] Hmknegr.
+    move : (mk_env_udiv_newer_gen Hmkudiv) => Hnewudiv.
+    case => <- _ <- _ //; move => Htt Hls1 Hls2; generalize Htt; rewrite newer_than_lit_tt_ff; move => Hff.
+    rewrite !interp_cnf_catrev.
+    move : (mk_env_neg_newer_res Hmkneg1 Htt Hls1) => Hgneg1.
+    move/andP : (mk_env_udiv_newer_res Hmkudiv (newer_than_lit_le_newer Htt Hnewneg1) Hgneg1 (newer_than_lits_le_newer Hls2 Hnewneg1)) => [Hgudiv _].
+    move : (mk_env_neg_sat Hmkneg1 Hff Hls1) => Hcnfneg1.
+    move : (mk_env_udiv_sat Hmkudiv (newer_than_lit_le_newer Htt Hnewneg1) Hgneg1 (newer_than_lits_le_newer Hls2 Hnewneg1)) => Hcnfudiv.
+    rewrite (mk_env_neg_sat Hmknegr (newer_than_lit_le_newer Htt (pos_leb_trans Hnewneg1 Hnewudiv)) Hgudiv).
+    rewrite (env_preserve_cnf (mk_env_neg_preserve Hmknegr) (mk_env_udiv_newer_cnf Hmkudiv (newer_than_lit_le_newer Htt Hnewneg1) Hgneg1 (newer_than_lits_le_newer Hls2 Hnewneg1))) Hcnfudiv.
+    rewrite (env_preserve_cnf (mk_env_neg_preserve Hmknegr) (newer_than_cnf_le_newer (mk_env_neg_newer_cnf Hmkneg1 Htt Hls1) Hnewudiv)).
+    rewrite (env_preserve_cnf (mk_env_udiv_preserve Hmkudiv) (mk_env_neg_newer_cnf Hmkneg1 Htt Hls1)) Hcnfneg1//.
+  - dcase (mk_env_xor E_neg1 g_neg1 ls2 (copy (size ls2) (splitmsl ls2).2)) => [[[[E_xor2] g_xor2] cs_xor2] rs_xor2] Hmkxor2.
+    dcase (mk_env_zeroextend (size (splitmsl ls2).1) E_xor2 g_xor2 [:: (splitmsl ls2).2]) => [[[[E_zext2] g_zext2] cs_zext2] rs_zext2] Hmkzext2.
+    dcase (mk_env_add E_zext2 g_zext2 rs_xor2 rs_zext2) => [[[[E_add2] g_add2] cs_add2] rs_add2] Hmkadd2.
+    dcase (mk_env_udiv E_add2 g_add2 rs_neg1 rs_add2) => [[[[[E_udiv] g_udiv] cs_udiv] lqs_udiv] lrs_udiv] Hmkudiv.
+    dcase (mk_env_neg E_udiv g_udiv lrs_udiv) => [[[[E_negr] g_negr] cs_negr] lrs_negr] Hmknegr.
+    move : (mk_env_xor_newer_gen Hmkxor2) => Hnewxor2.
+    move : (mk_env_zeroextend_newer_gen Hmkzext2) => Hnewzext2.
+    move : (mk_env_add_newer_gen Hmkadd2) => Hnewadd2.
+    move : (mk_env_udiv_newer_gen Hmkudiv) => Hnewudiv.
+    case => <- _ <- _ //; move => Htt Hls1 Hls2; generalize Htt; rewrite newer_than_lit_tt_ff; move => Hff.
+    rewrite !interp_cnf_catrev.
+    move : (mk_env_neg_newer_res Hmkneg1 Htt Hls1) => Hgneg1.
+    have Hnewcp : (newer_than_lits g_neg1 (copy (size ls2) (splitmsl ls2).2)).
+    {
+      move/andP : (newer_than_lits_splitmsl Htt Hls2) => [_ Hnewcp2].
+      exact : (newer_than_lits_le_newer (newer_than_lits_copy (size ls2) Hnewcp2) Hnewneg1).
+    }
+    have Hnewmsl: (newer_than_lits g_xor2 [:: (splitmsl ls2).2]).
+    {
+      move/andP : (newer_than_lits_splitmsl Htt Hls2) => [_ Hnewcp2].
+      exact : (newer_than_lits_le_newer (newer_than_lits_copy 1 Hnewcp2) (pos_leb_trans Hnewneg1 Hnewxor2)).
+    }
+    move : (mk_env_xor_newer_res Hmkxor2 (newer_than_lit_le_newer Htt Hnewneg1) (newer_than_lits_le_newer Hls2 Hnewneg1) Hnewcp) => Hgxor2.
+    move : (mk_env_zeroextend_newer_res Hmkzext2 (newer_than_lit_le_newer Htt (pos_leb_trans Hnewneg1 Hnewxor2)) Hnewmsl) => Hgzext2.
+    move : (mk_env_add_newer_res Hmkadd2) => Hgadd2.
+    move/andP : (mk_env_udiv_newer_res Hmkudiv (newer_than_lit_le_newer Htt (pos_leb_trans Hnewneg1 (pos_leb_trans Hnewxor2 (pos_leb_trans Hnewzext2 Hnewadd2)))) (newer_than_lits_le_newer Hgneg1 (pos_leb_trans Hnewxor2 (pos_leb_trans Hnewzext2 Hnewadd2))) Hgadd2) => [Hgudiv _].
+    move : (mk_env_neg_sat Hmkneg1 Htt Hls1) => Hcnfneg1.
+    move : (mk_env_xor_sat Hmkxor2 (newer_than_lit_le_newer Htt Hnewneg1) (newer_than_lits_le_newer Hls2 Hnewneg1) Hnewcp) => Hcnfxor2.
+    move : (mk_env_zeroextend_sat Hmkzext2 (newer_than_lit_le_newer Htt (pos_leb_trans Hnewneg1 Hnewxor2)) Hnewmsl) => Hcnfzext2.
+    move : (mk_env_add_sat Hmkadd2 (newer_than_lits_le_newer Hgxor2 Hnewzext2) Hgzext2 (newer_than_lit_le_newer Hff (pos_leb_trans Hnewneg1 (pos_leb_trans Hnewxor2 Hnewzext2)))) => Hcnfadd2.
+    move : (mk_env_udiv_sat Hmkudiv (newer_than_lit_le_newer Htt (pos_leb_trans Hnewneg1 (pos_leb_trans Hnewxor2 (pos_leb_trans Hnewzext2 Hnewadd2)))) (newer_than_lits_le_newer Hgneg1 (pos_leb_trans Hnewxor2 (pos_leb_trans Hnewzext2 Hnewadd2))) Hgadd2) => Hcnfudiv.
+    rewrite (mk_env_neg_sat Hmknegr (newer_than_lit_le_newer Htt (pos_leb_trans Hnewneg1 (pos_leb_trans Hnewxor2 (pos_leb_trans Hnewzext2 (pos_leb_trans Hnewadd2 Hnewudiv))))) Hgudiv).
+    rewrite (env_preserve_cnf (mk_env_neg_preserve Hmknegr) (mk_env_udiv_newer_cnf Hmkudiv (newer_than_lit_le_newer Htt (pos_leb_trans Hnewneg1 (pos_leb_trans Hnewxor2 (pos_leb_trans Hnewzext2 Hnewadd2)))) (newer_than_lits_le_newer Hgneg1 (pos_leb_trans Hnewxor2 (pos_leb_trans Hnewzext2 Hnewadd2))) Hgadd2)) Hcnfudiv.
+    rewrite (env_preserve_cnf (mk_env_neg_preserve Hmknegr) (newer_than_cnf_le_newer (mk_env_add_newer_cnf Hmkadd2 (newer_than_lits_le_newer Hgxor2 Hnewzext2) Hgzext2 (newer_than_lit_le_newer Hff (pos_leb_trans Hnewneg1 (pos_leb_trans Hnewxor2 Hnewzext2)))) Hnewudiv)).
+    rewrite (env_preserve_cnf (mk_env_udiv_preserve Hmkudiv) (mk_env_add_newer_cnf Hmkadd2 (newer_than_lits_le_newer Hgxor2 Hnewzext2) Hgzext2 (newer_than_lit_le_newer Hff (pos_leb_trans Hnewneg1 (pos_leb_trans Hnewxor2 Hnewzext2))))) Hcnfadd2.
+    rewrite (env_preserve_cnf (mk_env_neg_preserve Hmknegr) (newer_than_cnf_le_newer (mk_env_zeroextend_newer_cnf Hmkzext2 (newer_than_lit_le_newer Htt (pos_leb_trans Hnewneg1 Hnewxor2)) Hnewmsl) (pos_leb_trans Hnewadd2 Hnewudiv))).
+    rewrite (env_preserve_cnf (mk_env_udiv_preserve Hmkudiv) (newer_than_cnf_le_newer (mk_env_zeroextend_newer_cnf Hmkzext2 (newer_than_lit_le_newer Htt (pos_leb_trans Hnewneg1 Hnewxor2)) Hnewmsl) Hnewadd2)).
+    rewrite (env_preserve_cnf (mk_env_add_preserve Hmkadd2) (mk_env_zeroextend_newer_cnf Hmkzext2 (newer_than_lit_le_newer Htt (pos_leb_trans Hnewneg1 Hnewxor2)) Hnewmsl)) Hcnfzext2.
+    rewrite (env_preserve_cnf (mk_env_neg_preserve Hmknegr) (newer_than_cnf_le_newer (mk_env_xor_newer_cnf Hmkxor2 (newer_than_lit_le_newer Htt Hnewneg1) (newer_than_lits_le_newer Hls2 Hnewneg1) Hnewcp) (pos_leb_trans Hnewzext2 (pos_leb_trans Hnewadd2 Hnewudiv)))).
+    rewrite (env_preserve_cnf (mk_env_udiv_preserve Hmkudiv) (newer_than_cnf_le_newer (mk_env_xor_newer_cnf Hmkxor2 (newer_than_lit_le_newer Htt Hnewneg1) (newer_than_lits_le_newer Hls2 Hnewneg1) Hnewcp) (pos_leb_trans Hnewzext2 Hnewadd2))).
+    rewrite (env_preserve_cnf (mk_env_add_preserve Hmkadd2) (newer_than_cnf_le_newer (mk_env_xor_newer_cnf Hmkxor2 (newer_than_lit_le_newer Htt Hnewneg1) (newer_than_lits_le_newer Hls2 Hnewneg1) Hnewcp) Hnewzext2)).
+    rewrite (env_preserve_cnf (mk_env_zeroextend_preserve Hmkzext2) (mk_env_xor_newer_cnf Hmkxor2 (newer_than_lit_le_newer Htt Hnewneg1) (newer_than_lits_le_newer Hls2 Hnewneg1) Hnewcp)) Hcnfxor2.
+    rewrite (env_preserve_cnf (mk_env_neg_preserve Hmknegr) (newer_than_cnf_le_newer (mk_env_neg_newer_cnf Hmkneg1 Htt Hls1) (pos_leb_trans Hnewxor2 (pos_leb_trans Hnewzext2 (pos_leb_trans Hnewadd2 Hnewudiv))))).
+    rewrite (env_preserve_cnf (mk_env_udiv_preserve Hmkudiv) (newer_than_cnf_le_newer (mk_env_neg_newer_cnf Hmkneg1 Htt Hls1) (pos_leb_trans Hnewxor2 (pos_leb_trans Hnewzext2 Hnewadd2)))).
+    rewrite (env_preserve_cnf (mk_env_add_preserve Hmkadd2) (newer_than_cnf_le_newer (mk_env_neg_newer_cnf Hmkneg1 Htt Hls1) (pos_leb_trans Hnewxor2 Hnewzext2))).
+    rewrite (env_preserve_cnf (mk_env_zeroextend_preserve Hmkzext2) (newer_than_cnf_le_newer (mk_env_neg_newer_cnf Hmkneg1 Htt Hls1) Hnewxor2)).
+    rewrite (env_preserve_cnf (mk_env_xor_preserve Hmkxor2) (mk_env_neg_newer_cnf Hmkneg1 Htt Hls1)) Hcnfneg1//.
+  - dcase (mk_env_neg E g ls2) => [[[[E_abs2] g_abs2] cs_abs2] lrs_abs2] Hmkneg2.
+    dcase (mk_env_udiv E_abs2 g_abs2 ls1 lrs_abs2) => [[[[[E_udiv] g_udiv] cs_udiv] lqs_udiv]lrs_udiv] Hmkudiv.
+    move : (mk_env_neg_newer_gen Hmkneg2) => Hnewneg2.
+    case => <- _ <- _ //; move => Htt Hls1 Hls2; generalize Htt; rewrite newer_than_lit_tt_ff; move => Hff.
+    rewrite !interp_cnf_catrev.
+    move : (mk_env_neg_newer_res Hmkneg2 Htt Hls2) => Hgneg2.
+    rewrite (mk_env_udiv_sat Hmkudiv (newer_than_lit_le_newer Htt Hnewneg2) (newer_than_lits_le_newer Hls1 Hnewneg2) Hgneg2).
+    rewrite (env_preserve_cnf (mk_env_udiv_preserve Hmkudiv) (mk_env_neg_newer_cnf Hmkneg2 Htt Hls2)) (mk_env_neg_sat Hmkneg2 Hff Hls2)//.
+  - dcase (mk_env_udiv E g ls1 ls2) => [[[[[E_udiv] g_udiv] cs_udiv] lqs_udiv]lrs_udiv] Hmkudiv.
+    case => <- _ <- _ //; move => Htt Hls1 Hls2; generalize Htt; rewrite newer_than_lit_tt_ff; move => Hff.
+    rewrite (mk_env_udiv_sat Hmkudiv Htt Hls1 Hls2)//.
+  - dcase (mk_env_xor E g ls2 (copy (size ls2) (splitmsl ls2).2)) => [[[[E_xor2] g_xor2] cs_xor2] rs_xor2] Hmkxor2.
+    dcase (mk_env_zeroextend (size (splitmsl ls2).1) E_xor2 g_xor2 [:: (splitmsl ls2).2]) => [[[[E_zext2] g_zext2] cs_zext2] rs_zext2] Hmkzext2.
+    dcase (mk_env_add E_zext2 g_zext2 rs_xor2 rs_zext2) => [[[[E_add2] g_add2] cs_add2] rs_add2] Hmkadd2.
+    dcase (mk_env_udiv E_add2 g_add2 ls1 rs_add2) => [[[[[E_udiv] g_udiv] cs_udiv] lqs_udiv] lrs_udiv] Hmkudiv.
+    case => <- _ <- _ //; move => Htt Hls1 Hls2; generalize Htt; rewrite newer_than_lit_tt_ff; move => Hff.
+    rewrite !interp_cnf_catrev.
+    move : (mk_env_xor_newer_gen Hmkxor2) => Hnewxor2.
+    move : (mk_env_zeroextend_newer_gen Hmkzext2) => Hnewzext2.
+    move : (mk_env_add_newer_gen Hmkadd2) => Hnewadd2.
+    have Hnewcp : (newer_than_lits g (copy (size ls2) (splitmsl ls2).2)).
+    {
+      move/andP : (newer_than_lits_splitmsl Htt Hls2) => [_ Hnewcp2].
+      exact : (newer_than_lits_copy (size ls2) Hnewcp2).
+    }
+    have Hnewmsl: (newer_than_lits g_xor2 [:: (splitmsl ls2).2]).
+    {
+      move/andP : (newer_than_lits_splitmsl Htt Hls2) => [_ Hnewcp2].
+      exact : (newer_than_lits_le_newer (newer_than_lits_copy 1 Hnewcp2) Hnewxor2).
+    }
+    move : (pos_leb_trans Hnewxor2 (pos_leb_trans Hnewzext2 Hnewadd2)) => Hggadd2.
+    move : (mk_env_xor_newer_res Hmkxor2 Htt Hls2 Hnewcp) => Hgxor2.
+    move : (mk_env_zeroextend_newer_res Hmkzext2 (newer_than_lit_le_newer Htt Hnewxor2) Hnewmsl) => Hgzext2.
+    move : (mk_env_add_newer_res Hmkadd2) => Hgadd2.
+    move/andP : (mk_env_udiv_newer_res Hmkudiv (newer_than_lit_le_newer Htt Hggadd2) (newer_than_lits_le_newer Hls1 Hggadd2) Hgadd2) => [Hgudiv _].
+    move : (mk_env_xor_sat Hmkxor2 Htt Hls2 Hnewcp) => Hcnfxor2.
+    move : (mk_env_zeroextend_sat Hmkzext2 (newer_than_lit_le_newer Htt Hnewxor2) Hnewmsl) => Hcnfzext2.
+    move : (mk_env_add_sat Hmkadd2 (newer_than_lits_le_newer Hgxor2 Hnewzext2) Hgzext2 (newer_than_lit_le_newer Hff (pos_leb_trans Hnewxor2 Hnewzext2))) => Hcnfadd2.
+    rewrite (mk_env_udiv_sat Hmkudiv (newer_than_lit_le_newer Htt (pos_leb_trans Hnewxor2 (pos_leb_trans Hnewzext2 Hnewadd2))) (newer_than_lits_le_newer Hls1 Hggadd2) Hgadd2).
+    rewrite (env_preserve_cnf (mk_env_udiv_preserve Hmkudiv) (mk_env_add_newer_cnf Hmkadd2 (newer_than_lits_le_newer Hgxor2 Hnewzext2) Hgzext2 (newer_than_lit_le_newer Hff (pos_leb_trans Hnewxor2 Hnewzext2)))) Hcnfadd2.
+    rewrite (env_preserve_cnf (mk_env_udiv_preserve Hmkudiv) (newer_than_cnf_le_newer (mk_env_zeroextend_newer_cnf Hmkzext2 (newer_than_lit_le_newer Htt Hnewxor2) Hnewmsl) Hnewadd2)).
+    rewrite (env_preserve_cnf (mk_env_add_preserve Hmkadd2) (mk_env_zeroextend_newer_cnf Hmkzext2 (newer_than_lit_le_newer Htt Hnewxor2) Hnewmsl)) Hcnfzext2.
+    rewrite (env_preserve_cnf (mk_env_udiv_preserve Hmkudiv) (newer_than_cnf_le_newer (mk_env_xor_newer_cnf Hmkxor2 Htt Hls2 Hnewcp) (pos_leb_trans Hnewzext2 Hnewadd2))).
+    rewrite (env_preserve_cnf (mk_env_add_preserve Hmkadd2) (newer_than_cnf_le_newer (mk_env_xor_newer_cnf Hmkxor2 Htt Hls2 Hnewcp) Hnewzext2)).
+    rewrite (env_preserve_cnf (mk_env_zeroextend_preserve Hmkzext2) (mk_env_xor_newer_cnf Hmkxor2 Htt Hls2 Hnewcp)) Hcnfxor2//.
+  - dcase (mk_env_neg E_add g_add ls2) => [[[[E_abs2] g_abs2] cs_abs2] lrs_abs2] Hmkneg2.
+    dcase (mk_env_udiv E_abs2 g_abs2 rs_add lrs_abs2) => [[[[[E_udiv] g_udiv] cs_udiv] lqs_udiv]lrs_udiv] Hmkudiv.
+    dcase (mk_env_xor E_udiv g_udiv lrs_udiv (copy (size ls1) (splitmsl ls1).2)) => [[[[E_xorr] g_xorr] cs_xorr] rs_xorr] Hmkxorr.
+    dcase (mk_env_zeroextend (size (splitmsl ls1).1) E_xorr g_xorr [:: (splitmsl ls1).2]) => [[[[E_zextr] g_zextr] cs_zextr] rs_zextr] Hmkzextr.
+    dcase (mk_env_add E_zextr g_zextr rs_xorr rs_zextr) => [[[[E_addr] g_addr] cs_addr] rs_addr] Hmkaddr.
+    case => <- _ <- _ //; move => Htt Hls1 Hls2; generalize Htt; rewrite newer_than_lit_tt_ff; move => Hff.
+    rewrite !interp_cnf_catrev.
+    move : (mk_env_neg_newer_gen Hmkneg2) => Hnewneg2.
+    move : (mk_env_udiv_newer_gen Hmkudiv) => Hnewudiv.
+    move : (mk_env_xor_newer_gen Hmkxorr) => Hnewxorr.
+    move : (mk_env_zeroextend_newer_gen Hmkzextr) => Hnewzextr.
+    move : (mk_env_add_newer_gen Hmkaddr) => Hnewaddr.
+    have Hnewcp : (newer_than_lits g (copy (size ls1) (splitmsl ls1).2)).
+    {
+      move/andP : (newer_than_lits_splitmsl Htt Hls1) => [_ Hnewcp2].
+      exact : (newer_than_lits_copy (size ls1) Hnewcp2).
+    }
+    have Hnewmsl: (newer_than_lits g [:: (splitmsl ls1).2]).
+    {
+      move/andP : (newer_than_lits_splitmsl Htt Hls1) => [_ Hnewcp2].
+      exact : (newer_than_lits_copy 1 Hnewcp2) .
+    }
+    move : (pos_leb_trans Hnegls1 (pos_leb_trans Hnewneg2 (pos_leb_trans Hnewudiv Hnewxorr))) => Hggxorr.
+    move : (mk_env_xor_newer_res Hmkxor1 Htt Hls1 Hnewcp) => Hgxor1.
+    move : (mk_env_zeroextend_newer_res Hmkzext1 (newer_than_lit_le_newer Htt Hnewxor1) (newer_than_lits_le_newer Hnewmsl Hnewxor1)) => Hgzext1.
+    move : (mk_env_add_newer_res Hmkadd1) => Hgadd1.
+    move : (mk_env_neg_newer_res Hmkneg2 (newer_than_lit_le_newer Htt Hnegls1) (newer_than_lits_le_newer Hls2 Hnegls1)) => Hgneg2.
+    move/andP : (mk_env_udiv_newer_res Hmkudiv (newer_than_lit_le_newer Htt (pos_leb_trans Hnegls1 Hnewneg2)) (newer_than_lits_le_newer Hgadd1 Hnewneg2) Hgneg2) => [Hgudiv _].
+    move : (mk_env_xor_newer_res Hmkxorr (newer_than_lit_le_newer Htt (pos_leb_trans Hnegls1 (pos_leb_trans Hnewneg2 Hnewudiv))) Hgudiv (newer_than_lits_le_newer Hnewcp (pos_leb_trans Hnegls1 (pos_leb_trans Hnewneg2 Hnewudiv)))) => Hgxorr.
+    move : (mk_env_zeroextend_newer_res Hmkzextr (newer_than_lit_le_newer Htt (pos_leb_trans Hnegls1 (pos_leb_trans Hnewneg2 (pos_leb_trans Hnewudiv Hnewxorr)))) (newer_than_lits_le_newer Hnewmsl Hggxorr)) => Hgzextr.
+    move : (mk_env_xor_sat Hmkxorr (newer_than_lit_le_newer Htt (pos_leb_trans Hnegls1 (pos_leb_trans Hnewneg2 Hnewudiv))) Hgudiv (newer_than_lits_le_newer Hnewcp (pos_leb_trans Hnegls1 (pos_leb_trans Hnewneg2 Hnewudiv)))) => Hcnfxorr.
+    move : (mk_env_zeroextend_sat Hmkzextr (newer_than_lit_le_newer Htt (pos_leb_trans Hnegls1 (pos_leb_trans Hnewneg2 (pos_leb_trans Hnewudiv Hnewxorr)))) (newer_than_lits_le_newer Hnewmsl Hggxorr)) => Hcnfzextr.
+    move : (mk_env_udiv_sat Hmkudiv (newer_than_lit_le_newer Htt (pos_leb_trans Hnegls1 Hnewneg2)) (newer_than_lits_le_newer Hgadd1 Hnewneg2) Hgneg2) => Hcnfudiv.
+    rewrite (mk_env_add_sat Hmkaddr (newer_than_lits_le_newer Hgxorr Hnewzextr) Hgzextr (newer_than_lit_le_newer Hff (pos_leb_trans Hnegls1 (pos_leb_trans Hnewneg2 (pos_leb_trans Hnewudiv (pos_leb_trans Hnewxorr Hnewzextr)))))).
+    rewrite (env_preserve_cnf (mk_env_add_preserve Hmkaddr) (mk_env_zeroextend_newer_cnf Hmkzextr (newer_than_lit_le_newer Htt (pos_leb_trans Hnegls1 (pos_leb_trans Hnewneg2 (pos_leb_trans Hnewudiv Hnewxorr)))) (newer_than_lits_le_newer Hnewmsl Hggxorr))) Hcnfzextr.
+    rewrite (env_preserve_cnf (mk_env_add_preserve Hmkaddr) (newer_than_cnf_le_newer (mk_env_xor_newer_cnf Hmkxorr (newer_than_lit_le_newer Htt (pos_leb_trans Hnegls1 (pos_leb_trans Hnewneg2 Hnewudiv))) Hgudiv (newer_than_lits_le_newer Hnewcp (pos_leb_trans Hnegls1 (pos_leb_trans Hnewneg2 Hnewudiv)))) Hnewzextr)).
+    rewrite (env_preserve_cnf (mk_env_zeroextend_preserve Hmkzextr) (mk_env_xor_newer_cnf Hmkxorr (newer_than_lit_le_newer Htt (pos_leb_trans Hnegls1 (pos_leb_trans Hnewneg2 Hnewudiv))) Hgudiv (newer_than_lits_le_newer Hnewcp (pos_leb_trans Hnegls1 (pos_leb_trans Hnewneg2 Hnewudiv))))) Hcnfxorr.
+    rewrite (env_preserve_cnf (mk_env_add_preserve Hmkaddr) (newer_than_cnf_le_newer (mk_env_udiv_newer_cnf Hmkudiv (newer_than_lit_le_newer Htt (pos_leb_trans Hnegls1 Hnewneg2)) (newer_than_lits_le_newer Hgadd1 Hnewneg2) Hgneg2) (pos_leb_trans Hnewxorr Hnewzextr))).
+    rewrite (env_preserve_cnf (mk_env_zeroextend_preserve Hmkzextr) (newer_than_cnf_le_newer (mk_env_udiv_newer_cnf Hmkudiv (newer_than_lit_le_newer Htt (pos_leb_trans Hnegls1 Hnewneg2)) (newer_than_lits_le_newer Hgadd1 Hnewneg2) Hgneg2) Hnewxorr)).
+    rewrite (env_preserve_cnf (mk_env_xor_preserve Hmkxorr) (mk_env_udiv_newer_cnf Hmkudiv (newer_than_lit_le_newer Htt (pos_leb_trans Hnegls1 Hnewneg2)) (newer_than_lits_le_newer Hgadd1 Hnewneg2) Hgneg2)) Hcnfudiv.
+    rewrite (env_preserve_cnf (mk_env_add_preserve Hmkaddr) (newer_than_cnf_le_newer (mk_env_xor_newer_cnf Hmkxor1 Htt Hls1 Hnewcp) (pos_leb_trans Hnewzext1 (pos_leb_trans Hnewadd1 (pos_leb_trans Hnewneg2 (pos_leb_trans Hnewudiv (pos_leb_trans Hnewxorr Hnewzextr))))))).
+    rewrite (env_preserve_cnf (mk_env_zeroextend_preserve Hmkzextr) (newer_than_cnf_le_newer (mk_env_xor_newer_cnf Hmkxor1 Htt Hls1 Hnewcp) (pos_leb_trans Hnewzext1 (pos_leb_trans Hnewadd1 (pos_leb_trans Hnewneg2 (pos_leb_trans Hnewudiv Hnewxorr)))))).
+    rewrite (env_preserve_cnf (mk_env_xor_preserve Hmkxorr) (newer_than_cnf_le_newer (mk_env_xor_newer_cnf Hmkxor1 Htt Hls1 Hnewcp) (pos_leb_trans Hnewzext1 (pos_leb_trans Hnewadd1 (pos_leb_trans Hnewneg2 Hnewudiv))))).
+    rewrite (env_preserve_cnf (mk_env_udiv_preserve Hmkudiv) (newer_than_cnf_le_newer (mk_env_xor_newer_cnf Hmkxor1 Htt Hls1 Hnewcp) (pos_leb_trans Hnewzext1 (pos_leb_trans Hnewadd1 Hnewneg2)))).
+    rewrite (env_preserve_cnf (mk_env_neg_preserve Hmkneg2) (newer_than_cnf_le_newer (mk_env_xor_newer_cnf Hmkxor1 Htt Hls1 Hnewcp) (pos_leb_trans Hnewzext1 Hnewadd1))).
+    rewrite (env_preserve_cnf (mk_env_add_preserve Hmkadd1) (newer_than_cnf_le_newer (mk_env_xor_newer_cnf Hmkxor1 Htt Hls1 Hnewcp) Hnewzext1)).
+    rewrite (env_preserve_cnf (mk_env_zeroextend_preserve Hmkzext1) (mk_env_xor_newer_cnf Hmkxor1 Htt Hls1 Hnewcp)) (mk_env_xor_sat Hmkxor1 Htt Hls1 Hnewcp).
+    move : (mk_env_zeroextend_newer_cnf Hmkzext1 (newer_than_lit_le_newer Htt Hnewxor1) (newer_than_lits_le_newer Hnewmsl Hnewxor1)) => Hcszext1.
+    rewrite (env_preserve_cnf (mk_env_add_preserve Hmkaddr) (newer_than_cnf_le_newer Hcszext1 (pos_leb_trans Hnewadd1 (pos_leb_trans Hnewneg2 (pos_leb_trans Hnewudiv (pos_leb_trans Hnewxorr Hnewzextr)))))).
+    rewrite (env_preserve_cnf (mk_env_zeroextend_preserve Hmkzextr) (newer_than_cnf_le_newer Hcszext1 (pos_leb_trans Hnewadd1 (pos_leb_trans Hnewneg2 (pos_leb_trans Hnewudiv Hnewxorr))))).
+    rewrite (env_preserve_cnf (mk_env_xor_preserve Hmkxorr) (newer_than_cnf_le_newer Hcszext1 (pos_leb_trans Hnewadd1 (pos_leb_trans Hnewneg2 Hnewudiv)))).
+    rewrite (env_preserve_cnf (mk_env_udiv_preserve Hmkudiv) (newer_than_cnf_le_newer Hcszext1 (pos_leb_trans Hnewadd1 Hnewneg2))).
+    rewrite (env_preserve_cnf (mk_env_neg_preserve Hmkneg2) (newer_than_cnf_le_newer Hcszext1 Hnewadd1)).
+    rewrite (env_preserve_cnf (mk_env_add_preserve Hmkadd1) Hcszext1) (mk_env_zeroextend_sat Hmkzext1 (newer_than_lit_le_newer Htt Hnewxor1) (newer_than_lits_le_newer Hnewmsl Hnewxor1)).
+    move : (mk_env_add_newer_cnf Hmkadd1 (newer_than_lits_le_newer Hgxor1 Hnewzext1) Hgzext1 (newer_than_lit_le_newer Hff (pos_leb_trans Hnewxor1 Hnewzext1))) => Hcsadd1.
+    rewrite (env_preserve_cnf (mk_env_add_preserve Hmkaddr) (newer_than_cnf_le_newer Hcsadd1 (pos_leb_trans Hnewneg2 (pos_leb_trans Hnewudiv (pos_leb_trans Hnewxorr Hnewzextr))))).
+    rewrite (env_preserve_cnf (mk_env_zeroextend_preserve Hmkzextr) (newer_than_cnf_le_newer Hcsadd1 (pos_leb_trans Hnewneg2 (pos_leb_trans Hnewudiv Hnewxorr)))).
+    rewrite (env_preserve_cnf (mk_env_xor_preserve Hmkxorr) (newer_than_cnf_le_newer Hcsadd1 (pos_leb_trans Hnewneg2 Hnewudiv))).
+    rewrite (env_preserve_cnf (mk_env_udiv_preserve Hmkudiv) (newer_than_cnf_le_newer Hcsadd1 Hnewneg2)).
+    rewrite (env_preserve_cnf (mk_env_neg_preserve Hmkneg2) Hcsadd1) (mk_env_add_sat Hmkadd1 (newer_than_lits_le_newer Hgxor1 Hnewzext1) Hgzext1 (newer_than_lit_le_newer Hff (pos_leb_trans Hnewxor1 Hnewzext1))).
+    move : (mk_env_neg_sat Hmkneg2 (newer_than_lit_le_newer Hff Hnegls1) (newer_than_lits_le_newer Hls2 Hnegls1)) => Hcnfneg2.
+    move : (mk_env_neg_newer_cnf Hmkneg2 (newer_than_lit_le_newer Hff Hnegls1) (newer_than_lits_le_newer Hls2 Hnegls1)) => Hcsneg2.
+    rewrite (env_preserve_cnf (mk_env_add_preserve Hmkaddr) (newer_than_cnf_le_newer Hcsneg2 (pos_leb_trans Hnewudiv (pos_leb_trans Hnewxorr Hnewzextr)))).
+    rewrite (env_preserve_cnf (mk_env_zeroextend_preserve Hmkzextr) (newer_than_cnf_le_newer Hcsneg2 (pos_leb_trans Hnewudiv Hnewxorr))).
+    rewrite (env_preserve_cnf (mk_env_xor_preserve Hmkxorr) (newer_than_cnf_le_newer Hcsneg2 Hnewudiv)).
+    rewrite (env_preserve_cnf (mk_env_udiv_preserve Hmkudiv) Hcsneg2) Hcnfneg2//.
+  - dcase (mk_env_udiv E_add g_add rs_add ls2) => [[[[[E_udiv] g_udiv] cs_udiv] lqs_udiv]lrs_udiv] Hmkudiv.
+    dcase (mk_env_xor E_udiv g_udiv lrs_udiv (copy (size ls1) (splitmsl ls1).2)) => [[[[E_xorr] g_xorr] cs_xorr] rs_xorr] Hmkxorr.
+    dcase (mk_env_zeroextend (size (splitmsl ls1).1) E_xorr g_xorr [:: (splitmsl ls1).2]) => [[[[E_zextr] g_zextr] cs_zextr] rs_zextr] Hmkzextr.
+    dcase (mk_env_add E_zextr g_zextr rs_xorr rs_zextr) => [[[[E_addr] g_addr] cs_addr] rs_addr] Hmkaddr.
+    case => <- _ <- _ //; move => Htt Hls1 Hls2; generalize Htt; rewrite newer_than_lit_tt_ff; move => Hff.
+    rewrite !interp_cnf_catrev.
+    move : (mk_env_udiv_newer_gen Hmkudiv) => Hnewudiv.
+    move : (mk_env_xor_newer_gen Hmkxorr) => Hnewxorr.
+    move : (mk_env_zeroextend_newer_gen Hmkzextr) => Hnewzextr.
+    move : (mk_env_add_newer_gen Hmkaddr) => Hnewaddr.
+    have Hnewcp : (newer_than_lits g (copy (size ls1) (splitmsl ls1).2)).
+    {
+      move/andP : (newer_than_lits_splitmsl Htt Hls1) => [_ Hnewcp2].
+      exact : (newer_than_lits_copy (size ls1) Hnewcp2).
+    }
+    have Hnewmsl: (newer_than_lits g [:: (splitmsl ls1).2]).
+    {
+      move/andP : (newer_than_lits_splitmsl Htt Hls1) => [_ Hnewcp2].
+      exact : (newer_than_lits_copy 1 Hnewcp2) .
+    }
+    move : (pos_leb_trans Hnegls1 (pos_leb_trans Hnewudiv Hnewxorr)) => Hggxorr.
+    move : (mk_env_xor_newer_res Hmkxor1 Htt Hls1 Hnewcp) => Hgxor1.
+    move : (mk_env_zeroextend_newer_res Hmkzext1 (newer_than_lit_le_newer Htt Hnewxor1) (newer_than_lits_le_newer Hnewmsl Hnewxor1)) => Hgzext1.
+    move : (mk_env_add_newer_res Hmkadd1) => Hgadd1.
+    move/andP : (mk_env_udiv_newer_res Hmkudiv (newer_than_lit_le_newer Htt Hnegls1) Hgadd1 (newer_than_lits_le_newer Hls2 Hnegls1)) => [Hgudiv _].
+    move : (mk_env_xor_newer_res Hmkxorr (newer_than_lit_le_newer Htt (pos_leb_trans Hnegls1 Hnewudiv)) Hgudiv (newer_than_lits_le_newer Hnewcp (pos_leb_trans Hnegls1 Hnewudiv))) => Hgxorr.
+    move : (mk_env_zeroextend_newer_res Hmkzextr (newer_than_lit_le_newer Htt (pos_leb_trans Hnegls1 (pos_leb_trans Hnewudiv Hnewxorr))) (newer_than_lits_le_newer Hnewmsl Hggxorr)) => Hgzextr.
+    move : (mk_env_xor_sat Hmkxorr (newer_than_lit_le_newer Htt (pos_leb_trans Hnegls1 Hnewudiv)) Hgudiv (newer_than_lits_le_newer Hnewcp (pos_leb_trans Hnegls1 Hnewudiv))) => Hcnfxorr.
+    move : (mk_env_zeroextend_sat Hmkzextr (newer_than_lit_le_newer Htt (pos_leb_trans Hnegls1 (pos_leb_trans Hnewudiv Hnewxorr))) (newer_than_lits_le_newer Hnewmsl Hggxorr)) => Hcnfzextr.
+    move : (mk_env_udiv_sat Hmkudiv (newer_than_lit_le_newer Htt Hnegls1) Hgadd1 (newer_than_lits_le_newer Hls2 Hnegls1)) => Hcnfudiv.
+    move : (mk_env_xor_newer_cnf Hmkxor1 Htt Hls1 Hnewcp) => Hcsxor1.
+    move : (mk_env_xor_sat Hmkxor1 Htt Hls1 Hnewcp) => Hcnfxor1.
+    rewrite (env_preserve_cnf (mk_env_add_preserve Hmkaddr) (newer_than_cnf_le_newer Hcsxor1 (pos_leb_trans Hnewzext1 (pos_leb_trans Hnewadd1 (pos_leb_trans Hnewudiv (pos_leb_trans Hnewxorr Hnewzextr)))))).
+    rewrite (env_preserve_cnf (mk_env_zeroextend_preserve Hmkzextr) (newer_than_cnf_le_newer Hcsxor1 (pos_leb_trans Hnewzext1 (pos_leb_trans Hnewadd1 (pos_leb_trans Hnewudiv Hnewxorr))))).
+    rewrite (env_preserve_cnf (mk_env_xor_preserve Hmkxorr) (newer_than_cnf_le_newer Hcsxor1 (pos_leb_trans Hnewzext1 (pos_leb_trans Hnewadd1 Hnewudiv)))).
+    rewrite (env_preserve_cnf (mk_env_udiv_preserve Hmkudiv) (newer_than_cnf_le_newer Hcsxor1 (pos_leb_trans Hnewzext1 Hnewadd1))).
+    rewrite (env_preserve_cnf (mk_env_add_preserve Hmkadd1) (newer_than_cnf_le_newer Hcsxor1 Hnewzext1)).
+    rewrite (env_preserve_cnf (mk_env_zeroextend_preserve Hmkzext1) Hcsxor1) Hcnfxor1.
+    move : (mk_env_zeroextend_newer_cnf Hmkzext1 (newer_than_lit_le_newer Htt Hnewxor1) (newer_than_lits_le_newer Hnewmsl Hnewxor1)) => Hcszext1.
+    move : (mk_env_zeroextend_sat Hmkzext1 (newer_than_lit_le_newer Htt Hnewxor1) (newer_than_lits_le_newer Hnewmsl Hnewxor1)) => Hcnfzext1.
+    rewrite (env_preserve_cnf (mk_env_add_preserve Hmkaddr) (newer_than_cnf_le_newer Hcszext1 (pos_leb_trans Hnewadd1 (pos_leb_trans Hnewudiv (pos_leb_trans Hnewxorr Hnewzextr))))).
+    rewrite (env_preserve_cnf (mk_env_zeroextend_preserve Hmkzextr) (newer_than_cnf_le_newer Hcszext1 (pos_leb_trans Hnewadd1 (pos_leb_trans Hnewudiv Hnewxorr)))).
+    rewrite (env_preserve_cnf (mk_env_xor_preserve Hmkxorr) (newer_than_cnf_le_newer Hcszext1 (pos_leb_trans Hnewadd1 Hnewudiv))).
+    rewrite (env_preserve_cnf (mk_env_udiv_preserve Hmkudiv) (newer_than_cnf_le_newer Hcszext1 Hnewadd1)).
+    rewrite (env_preserve_cnf (mk_env_add_preserve Hmkadd1) Hcszext1) Hcnfzext1.
+    move : (mk_env_add_newer_cnf Hmkadd1 (newer_than_lits_le_newer Hgxor1 Hnewzext1) Hgzext1 (newer_than_lit_le_newer Hff (pos_leb_trans Hnewxor1 Hnewzext1))) => Hcsadd1.
+    move : (mk_env_add_sat Hmkadd1 (newer_than_lits_le_newer Hgxor1 Hnewzext1) Hgzext1 (newer_than_lit_le_newer Hff (pos_leb_trans Hnewxor1 Hnewzext1))) => Hcnfadd1.
+    rewrite (env_preserve_cnf (mk_env_add_preserve Hmkaddr) (newer_than_cnf_le_newer Hcsadd1 (pos_leb_trans Hnewudiv (pos_leb_trans Hnewxorr Hnewzextr)))).
+    rewrite (env_preserve_cnf (mk_env_zeroextend_preserve Hmkzextr) (newer_than_cnf_le_newer Hcsadd1 (pos_leb_trans Hnewudiv Hnewxorr))).
+    rewrite (env_preserve_cnf (mk_env_xor_preserve Hmkxorr) (newer_than_cnf_le_newer Hcsadd1 Hnewudiv)).
+    rewrite (env_preserve_cnf (mk_env_udiv_preserve Hmkudiv) Hcsadd1) Hcnfadd1/=.
+    move : (mk_env_udiv_newer_cnf Hmkudiv (newer_than_lit_le_newer Htt Hnegls1) Hgadd1 (newer_than_lits_le_newer Hls2 Hnegls1)) => Hcsudiv.
+    rewrite (env_preserve_cnf (mk_env_add_preserve Hmkaddr) (newer_than_cnf_le_newer Hcsudiv (pos_leb_trans Hnewxorr Hnewzextr))).
+    rewrite (env_preserve_cnf (mk_env_zeroextend_preserve Hmkzextr) (newer_than_cnf_le_newer Hcsudiv Hnewxorr)).
+    rewrite (env_preserve_cnf (mk_env_xor_preserve Hmkxorr) Hcsudiv) Hcnfudiv.
+    move : (mk_env_zeroextend_newer_cnf Hmkzextr (newer_than_lit_le_newer Htt (pos_leb_trans Hnegls1 (pos_leb_trans Hnewudiv Hnewxorr))) (newer_than_lits_le_newer Hnewmsl Hggxorr)) => Hcszextr.
+    rewrite (env_preserve_cnf (mk_env_add_preserve Hmkaddr) Hcszextr) Hcnfzextr.
+    move : (mk_env_xor_newer_cnf Hmkxorr (newer_than_lit_le_newer Htt (pos_leb_trans Hnegls1 Hnewudiv)) Hgudiv (newer_than_lits_le_newer Hnewcp (pos_leb_trans Hnegls1 Hnewudiv))) => Hcsxorr.
+    rewrite (env_preserve_cnf (mk_env_add_preserve Hmkaddr) (newer_than_cnf_le_newer Hcsxorr Hnewzextr)).
+    rewrite (env_preserve_cnf (mk_env_zeroextend_preserve Hmkzextr) Hcsxorr) Hcnfxorr.
+    rewrite (mk_env_add_sat Hmkaddr (newer_than_lits_le_newer Hgxorr Hnewzextr) Hgzextr (newer_than_lit_le_newer Hff (pos_leb_trans Hggxorr Hnewzextr)))//.
+  - dcase (mk_env_xor E_add g_add ls2 (copy (size ls2) (splitmsl ls2).2)) => [[[[E_xor2] g_xor2] cs_xor2] rs_xor2] Hmkxor2.
+    dcase (mk_env_zeroextend (size (splitmsl ls2).1) E_xor2 g_xor2 [:: (splitmsl ls2).2]) => [[[[E_zext2] g_zext2] cs_zext2] rs_zext2] Hmkzext2.
+    dcase (mk_env_add E_zext2 g_zext2 rs_xor2 rs_zext2) => [[[[E_abs2] g_abs2] cs_abs2] lrs_abs2] Hmkadd2.
+    dcase (mk_env_udiv E_abs2 g_abs2 rs_add lrs_abs2) => [[[[[E_udiv] g_udiv] cs_udiv] lqs_udiv]lrs_udiv] Hmkudiv.
+    dcase (mk_env_xor E_udiv g_udiv lrs_udiv (copy (size ls1) (splitmsl ls1).2)) => [[[[E_xorr] g_xorr] cs_xorr] rs_xorr] Hmkxorr.
+    dcase (mk_env_zeroextend (size (splitmsl ls1).1) E_xorr g_xorr [:: (splitmsl ls1).2]) => [[[[E_zextr] g_zextr] cs_zextr] rs_zextr] Hmkzextr.
+    dcase (mk_env_add E_zextr g_zextr rs_xorr rs_zextr) => [[[[E_addr] g_addr] cs_addr] rs_addr] Hmkaddr.
+    case => <- _ <- _ //; move => Htt Hls1 Hls2; generalize Htt; rewrite newer_than_lit_tt_ff; move => Hff.
+    rewrite !interp_cnf_catrev.
+    move : (mk_env_xor_newer_gen Hmkxor2) => Hnewxor2. 
+    move : (mk_env_zeroextend_newer_gen Hmkzext2) => Hnewzext2.
+    move : (mk_env_add_newer_gen Hmkadd2) => Hnewadd2.
+    move : (mk_env_udiv_newer_gen Hmkudiv) => Hnewudiv.
+    move : (mk_env_xor_newer_gen Hmkxorr) => Hnewxorr.
+    move : (mk_env_zeroextend_newer_gen Hmkzextr) => Hnewzextr.
+    move : (mk_env_add_newer_gen Hmkaddr) => Hnewaddr.
+    have Hnewcp : (newer_than_lits g (copy (size ls1) (splitmsl ls1).2)).
+    {
+      move/andP : (newer_than_lits_splitmsl Htt Hls1) => [_ Hnewc].
+      exact : (newer_than_lits_copy (size ls1) Hnewc).
+    }
+    have Hnewmsl: (newer_than_lits g [:: (splitmsl ls1).2]).
+    {
+      move/andP : (newer_than_lits_splitmsl Htt Hls1) => [_ Hnewc].
+      exact : (newer_than_lits_copy 1 Hnewc).
+    }
+    have Hnewcp2 : (newer_than_lits g (copy (size ls2) (splitmsl ls2).2)).
+    {
+      move/andP : (newer_than_lits_splitmsl Htt Hls2) => [_ Hnewc].
+      exact : (newer_than_lits_copy (size ls2) Hnewc). 
+    }
+    have Hnewmsl2 : (newer_than_lits g [:: (splitmsl ls2).2]).
+    {
+      move/andP : (newer_than_lits_splitmsl Htt Hls2) => [_ Hnewc].
+      exact : (newer_than_lits_copy 1 Hnewc) .
+    }
+    move : (pos_leb_trans Hnewxor2 (pos_leb_trans Hnewzext2 Hnewadd2)) => Hnegls2.
+    move : (pos_leb_trans Hnegls1 (pos_leb_trans Hnegls2 (pos_leb_trans Hnewudiv Hnewxorr))) => Hggxorr.
+    move : (mk_env_xor_newer_res Hmkxor1 Htt Hls1 Hnewcp) => Hgxor1.
+    move : (mk_env_zeroextend_newer_res Hmkzext1 (newer_than_lit_le_newer Htt Hnewxor1) (newer_than_lits_le_newer Hnewmsl Hnewxor1)) => Hgzext1.
+    move : (mk_env_add_newer_res Hmkadd1) => Hgadd1.
+    move : (mk_env_xor_newer_res Hmkxor2 (newer_than_lit_le_newer Htt Hnegls1) (newer_than_lits_le_newer Hls2 Hnegls1) (newer_than_lits_le_newer Hnewcp2 Hnegls1)) => Hgxor2.
+    move : (mk_env_zeroextend_newer_res Hmkzext2 (newer_than_lit_le_newer Htt (pos_leb_trans Hnegls1 Hnewxor2)) (newer_than_lits_le_newer Hnewmsl2 (pos_leb_trans Hnegls1 Hnewxor2))) => Hgzext2.
+    move : (mk_env_add_newer_res Hmkadd2) => Hgadd2.
+    move/andP : (mk_env_udiv_newer_res Hmkudiv (newer_than_lit_le_newer Htt (pos_leb_trans Hnegls1 Hnegls2)) (newer_than_lits_le_newer Hgadd1 Hnegls2) Hgadd2) => [Hgudiv _].
+    move : (mk_env_xor_newer_res Hmkxorr (newer_than_lit_le_newer Htt (pos_leb_trans (pos_leb_trans Hnegls1 Hnegls2) Hnewudiv)) Hgudiv (newer_than_lits_le_newer Hnewcp (pos_leb_trans (pos_leb_trans Hnegls1 Hnegls2) Hnewudiv))) => Hgxorr.
+    move : (mk_env_zeroextend_newer_res Hmkzextr (newer_than_lit_le_newer Htt (pos_leb_trans Hnegls1 (pos_leb_trans Hnegls2 (pos_leb_trans Hnewudiv Hnewxorr)))) (newer_than_lits_le_newer Hnewmsl Hggxorr)) => Hgzextr.
+    move : (mk_env_xor_sat Hmkxorr (newer_than_lit_le_newer Htt (pos_leb_trans Hnegls1 (pos_leb_trans Hnegls2 Hnewudiv))) Hgudiv (newer_than_lits_le_newer Hnewcp (pos_leb_trans Hnegls1 (pos_leb_trans Hnegls2 Hnewudiv)))) => Hcnfxorr.
+    move : (mk_env_zeroextend_sat Hmkzextr (newer_than_lit_le_newer Htt (pos_leb_trans Hnegls1 (pos_leb_trans Hnegls2 (pos_leb_trans Hnewudiv Hnewxorr)))) (newer_than_lits_le_newer Hnewmsl Hggxorr)) => Hcnfzextr.
+    move : (mk_env_udiv_sat Hmkudiv (newer_than_lit_le_newer Htt (pos_leb_trans Hnegls1 Hnegls2)) (newer_than_lits_le_newer Hgadd1 Hnegls2) Hgadd2) => Hcnfudiv.
+    move : (mk_env_xor_newer_cnf Hmkxor1 Htt Hls1 Hnewcp) => Hcsxor1.
+    move : (mk_env_xor_sat Hmkxor1 Htt Hls1 Hnewcp) => Hcnfxor1.
+    rewrite (env_preserve_cnf (mk_env_add_preserve Hmkaddr) (newer_than_cnf_le_newer Hcsxor1 (pos_leb_trans Hnewzext1 (pos_leb_trans Hnewadd1 (pos_leb_trans Hnegls2 (pos_leb_trans Hnewudiv (pos_leb_trans Hnewxorr Hnewzextr))))))).
+    rewrite (env_preserve_cnf (mk_env_zeroextend_preserve Hmkzextr) (newer_than_cnf_le_newer Hcsxor1 (pos_leb_trans Hnewzext1 (pos_leb_trans Hnewadd1 (pos_leb_trans Hnegls2 (pos_leb_trans Hnewudiv Hnewxorr)))))).
+    rewrite (env_preserve_cnf (mk_env_xor_preserve Hmkxorr) (newer_than_cnf_le_newer Hcsxor1 (pos_leb_trans Hnewzext1 (pos_leb_trans Hnewadd1 (pos_leb_trans Hnegls2 Hnewudiv))))).
+    rewrite (env_preserve_cnf (mk_env_udiv_preserve Hmkudiv) (newer_than_cnf_le_newer Hcsxor1 (pos_leb_trans Hnewzext1 (pos_leb_trans Hnewadd1 Hnegls2)))).
+    rewrite (env_preserve_cnf (mk_env_add_preserve Hmkadd2) (newer_than_cnf_le_newer Hcsxor1 (pos_leb_trans Hnewzext1 (pos_leb_trans Hnewadd1 (pos_leb_trans Hnewxor2 Hnewzext2))))).
+    rewrite (env_preserve_cnf (mk_env_zeroextend_preserve Hmkzext2) (newer_than_cnf_le_newer Hcsxor1 (pos_leb_trans Hnewzext1 (pos_leb_trans Hnewadd1 Hnewxor2)))).
+    rewrite (env_preserve_cnf (mk_env_xor_preserve Hmkxor2) (newer_than_cnf_le_newer Hcsxor1 (pos_leb_trans Hnewzext1 Hnewadd1))).
+    rewrite (env_preserve_cnf (mk_env_add_preserve Hmkadd1) (newer_than_cnf_le_newer Hcsxor1 Hnewzext1)).
+    rewrite (env_preserve_cnf (mk_env_zeroextend_preserve Hmkzext1) Hcsxor1) Hcnfxor1.
+    move : (mk_env_zeroextend_newer_cnf Hmkzext1 (newer_than_lit_le_newer Htt Hnewxor1) (newer_than_lits_le_newer Hnewmsl Hnewxor1)) => Hcszext1.
+    move : (mk_env_zeroextend_sat Hmkzext1 (newer_than_lit_le_newer Htt Hnewxor1) (newer_than_lits_le_newer Hnewmsl Hnewxor1)) => Hcnfzext1.
+    rewrite (env_preserve_cnf (mk_env_add_preserve Hmkaddr) (newer_than_cnf_le_newer Hcszext1 (pos_leb_trans Hnewadd1 (pos_leb_trans Hnegls2 (pos_leb_trans Hnewudiv (pos_leb_trans Hnewxorr Hnewzextr)))))).
+    rewrite (env_preserve_cnf (mk_env_zeroextend_preserve Hmkzextr) (newer_than_cnf_le_newer Hcszext1 (pos_leb_trans Hnewadd1 (pos_leb_trans Hnegls2 (pos_leb_trans Hnewudiv Hnewxorr))))).
+    rewrite (env_preserve_cnf (mk_env_xor_preserve Hmkxorr) (newer_than_cnf_le_newer Hcszext1 (pos_leb_trans Hnewadd1 (pos_leb_trans Hnegls2 Hnewudiv)))).
+    rewrite (env_preserve_cnf (mk_env_udiv_preserve Hmkudiv) (newer_than_cnf_le_newer Hcszext1 (pos_leb_trans Hnewadd1 Hnegls2))).
+    rewrite (env_preserve_cnf (mk_env_add_preserve Hmkadd2) (newer_than_cnf_le_newer Hcszext1 (pos_leb_trans Hnewadd1 (pos_leb_trans Hnewxor2 Hnewzext2)))).
+    rewrite (env_preserve_cnf (mk_env_zeroextend_preserve Hmkzext2) (newer_than_cnf_le_newer Hcszext1 (pos_leb_trans Hnewadd1 Hnewxor2))).
+    rewrite (env_preserve_cnf (mk_env_xor_preserve Hmkxor2) (newer_than_cnf_le_newer Hcszext1 Hnewadd1)).
+    rewrite (env_preserve_cnf (mk_env_add_preserve Hmkadd1) Hcszext1) Hcnfzext1.
+    move : (mk_env_add_newer_cnf Hmkadd1 (newer_than_lits_le_newer Hgxor1 Hnewzext1) Hgzext1 (newer_than_lit_le_newer Hff (pos_leb_trans Hnewxor1 Hnewzext1))) => Hcsadd1.
+    move : (mk_env_add_sat Hmkadd1 (newer_than_lits_le_newer Hgxor1 Hnewzext1) Hgzext1 (newer_than_lit_le_newer Hff (pos_leb_trans Hnewxor1 Hnewzext1))) => Hcnfadd1.
+    rewrite (env_preserve_cnf (mk_env_add_preserve Hmkaddr) (newer_than_cnf_le_newer Hcsadd1 (pos_leb_trans Hnegls2 (pos_leb_trans Hnewudiv (pos_leb_trans Hnewxorr Hnewzextr))))).
+    rewrite (env_preserve_cnf (mk_env_zeroextend_preserve Hmkzextr) (newer_than_cnf_le_newer Hcsadd1 (pos_leb_trans Hnegls2 (pos_leb_trans Hnewudiv Hnewxorr)))).
+    rewrite (env_preserve_cnf (mk_env_xor_preserve Hmkxorr) (newer_than_cnf_le_newer Hcsadd1 (pos_leb_trans Hnegls2 Hnewudiv))).
+    rewrite (env_preserve_cnf (mk_env_udiv_preserve Hmkudiv) (newer_than_cnf_le_newer Hcsadd1 Hnegls2)).
+    rewrite (env_preserve_cnf (mk_env_add_preserve Hmkadd2) (newer_than_cnf_le_newer Hcsadd1 (pos_leb_trans Hnewxor2 Hnewzext2))).
+    rewrite (env_preserve_cnf (mk_env_zeroextend_preserve Hmkzext2) (newer_than_cnf_le_newer Hcsadd1 Hnewxor2)).
+    rewrite (env_preserve_cnf (mk_env_xor_preserve Hmkxor2) Hcsadd1) Hcnfadd1/=.
+    move : (mk_env_udiv_newer_cnf Hmkudiv (newer_than_lit_le_newer Htt (pos_leb_trans Hnegls1 Hnegls2)) (newer_than_lits_le_newer Hgadd1 Hnegls2) Hgadd2) => Hcsudiv.
+    rewrite (env_preserve_cnf (mk_env_add_preserve Hmkaddr) (newer_than_cnf_le_newer Hcsudiv (pos_leb_trans Hnewxorr Hnewzextr))).
+    rewrite (env_preserve_cnf (mk_env_zeroextend_preserve Hmkzextr) (newer_than_cnf_le_newer Hcsudiv Hnewxorr)).
+    rewrite (env_preserve_cnf (mk_env_xor_preserve Hmkxorr) Hcsudiv) Hcnfudiv.
+    move : (mk_env_zeroextend_newer_cnf Hmkzextr (newer_than_lit_le_newer Htt (pos_leb_trans Hnegls1 (pos_leb_trans Hnegls2 (pos_leb_trans Hnewudiv Hnewxorr)))) (newer_than_lits_le_newer Hnewmsl Hggxorr)) => Hcszextr.
+    rewrite (env_preserve_cnf (mk_env_add_preserve Hmkaddr) Hcszextr) Hcnfzextr.
+    move : (mk_env_xor_newer_cnf Hmkxorr (newer_than_lit_le_newer Htt (pos_leb_trans Hnegls1 (pos_leb_trans Hnegls2 Hnewudiv))) Hgudiv (newer_than_lits_le_newer Hnewcp (pos_leb_trans Hnegls1 (pos_leb_trans Hnegls2 Hnewudiv)))) => Hcsxorr.
+    rewrite (env_preserve_cnf (mk_env_add_preserve Hmkaddr) (newer_than_cnf_le_newer Hcsxorr Hnewzextr)).
+    rewrite (env_preserve_cnf (mk_env_zeroextend_preserve Hmkzextr) Hcsxorr) Hcnfxorr.
+    rewrite (mk_env_add_sat Hmkaddr (newer_than_lits_le_newer Hgxorr Hnewzextr) Hgzextr (newer_than_lit_le_newer Hff (pos_leb_trans Hggxorr Hnewzextr))).
+    move : (mk_env_xor_sat Hmkxor2 (newer_than_lit_le_newer Htt Hnegls1) (newer_than_lits_le_newer Hls2 Hnegls1) (newer_than_lits_le_newer Hnewcp2 Hnegls1)) => Hcnfxor2.
+    move : (mk_env_xor_newer_cnf Hmkxor2 (newer_than_lit_le_newer Htt Hnegls1) (newer_than_lits_le_newer Hls2 Hnegls1) (newer_than_lits_le_newer Hnewcp2 Hnegls1)) => Hcsxor2.
+    rewrite (env_preserve_cnf (mk_env_add_preserve Hmkaddr) (newer_than_cnf_le_newer Hcsxor2 (pos_leb_trans Hnewzext2 (pos_leb_trans Hnewadd2 (pos_leb_trans Hnewudiv (pos_leb_trans Hnewxorr Hnewzextr)))))).
+    rewrite (env_preserve_cnf (mk_env_zeroextend_preserve Hmkzextr) (newer_than_cnf_le_newer Hcsxor2 (pos_leb_trans Hnewzext2 (pos_leb_trans Hnewadd2 (pos_leb_trans Hnewudiv Hnewxorr))))).
+    rewrite (env_preserve_cnf (mk_env_xor_preserve Hmkxorr) (newer_than_cnf_le_newer Hcsxor2 (pos_leb_trans Hnewzext2 (pos_leb_trans Hnewadd2 Hnewudiv)))).
+    rewrite (env_preserve_cnf (mk_env_udiv_preserve Hmkudiv) (newer_than_cnf_le_newer Hcsxor2 (pos_leb_trans Hnewzext2 Hnewadd2))).
+    rewrite (env_preserve_cnf (mk_env_add_preserve Hmkadd2) (newer_than_cnf_le_newer Hcsxor2 Hnewzext2)).
+    rewrite (env_preserve_cnf (mk_env_zeroextend_preserve Hmkzext2) Hcsxor2) Hcnfxor2.
+    move : (mk_env_zeroextend_newer_cnf Hmkzext2 (newer_than_lit_le_newer Htt (pos_leb_trans Hnegls1 Hnewxor2)) (newer_than_lits_le_newer Hnewmsl2 (pos_leb_trans Hnegls1 Hnewxor2))) => Hcszext2.
+    move : (mk_env_zeroextend_sat Hmkzext2 (newer_than_lit_le_newer Htt (pos_leb_trans Hnegls1 Hnewxor2)) (newer_than_lits_le_newer Hnewmsl2 (pos_leb_trans Hnegls1 Hnewxor2))) => Hcnfzext2.
+    rewrite (env_preserve_cnf (mk_env_add_preserve Hmkaddr) (newer_than_cnf_le_newer Hcszext2 (pos_leb_trans Hnewadd2 (pos_leb_trans Hnewudiv (pos_leb_trans Hnewxorr Hnewzextr))))).
+    rewrite (env_preserve_cnf (mk_env_zeroextend_preserve Hmkzextr) (newer_than_cnf_le_newer Hcszext2 (pos_leb_trans Hnewadd2 (pos_leb_trans Hnewudiv Hnewxorr)))).
+    rewrite (env_preserve_cnf (mk_env_xor_preserve Hmkxorr) (newer_than_cnf_le_newer Hcszext2 (pos_leb_trans Hnewadd2 Hnewudiv))).
+    rewrite (env_preserve_cnf (mk_env_udiv_preserve Hmkudiv) (newer_than_cnf_le_newer Hcszext2 Hnewadd2)).
+    rewrite (env_preserve_cnf (mk_env_add_preserve Hmkadd2) Hcszext2) Hcnfzext2.
+    move : (mk_env_add_sat Hmkadd2 (newer_than_lits_le_newer Hgxor2 Hnewzext2) Hgzext2 (newer_than_lit_le_newer Hff (pos_leb_trans Hnegls1 (pos_leb_trans Hnewxor2 Hnewzext2)))) => Hcnfadd2.
+    move : (mk_env_add_newer_cnf Hmkadd2 (newer_than_lits_le_newer Hgxor2 Hnewzext2) Hgzext2 (newer_than_lit_le_newer Hff (pos_leb_trans Hnegls1 (pos_leb_trans Hnewxor2 Hnewzext2)))) => Hcsadd2.
+    rewrite (env_preserve_cnf (mk_env_add_preserve Hmkaddr) (newer_than_cnf_le_newer Hcsadd2 (pos_leb_trans Hnewudiv (pos_leb_trans Hnewxorr Hnewzextr)))).
+    rewrite (env_preserve_cnf (mk_env_zeroextend_preserve Hmkzextr) (newer_than_cnf_le_newer Hcsadd2 (pos_leb_trans Hnewudiv Hnewxorr))).
+    rewrite (env_preserve_cnf (mk_env_xor_preserve Hmkxorr) (newer_than_cnf_le_newer Hcsadd2 Hnewudiv)).
+    rewrite (env_preserve_cnf (mk_env_udiv_preserve Hmkudiv) Hcsadd2) Hcnfadd2//.
+Qed.
+
+    (* Lemma bit_blast_sdiv_correct g ls1 ls2 g' cs qlrs rlrs E bs1 bs2 : *)
 (*   bit_blast_sdiv g ls1 ls2 = (g', cs, qlrs, rlrs) -> *)
 (*   size ls1 = size ls2 -> *)
 (*   0 < size ls2 -> *)
